Start compiling dynamic Matches

src/compiler.ml
@@ -1,3 +1,11 @@
+let rec fold_right_trace : 'a 'acc. ('a -> 'acc -> 'acc) -> 'a list -> 'acc -> 'acc list = fun f l acc ->
+  match l with
+  | [] -> [acc]
+  | a :: l' ->
+    match fold_right_trace f l' acc with
+    | acc_1 :: accs -> f a acc_1 :: accs
+    | _ -> assert false
+
 let reduce_right (type a) (f : a -> a -> a) (l : a list) : a =
   List.fold_right f (CList.drop_last l) (CList.last l)
 
@@ -13,6 +21,24 @@ let rec seq_product_list (seqs : 'a Seq.t list) : 'a list Seq.t =
 
 let seq_product_array (seqs : 'a Seq.t array) : 'a array Seq.t =
   seqs |> Array.to_list |> seq_product_list |> Seq.map Array.of_list
+
+let rec seq_zip_strict : 'a 'b. 'a Seq.t -> 'b Seq.t -> ('a * 'b) Seq.t = fun xs ys ->
+  fun () ->
+    match xs (), ys () with
+    | Nil, Nil -> Nil
+    | Cons (x, xs), Cons (y, ys) -> Cons ((x, y), seq_zip_strict xs ys)
+    | _, _ -> failwith "sequences have different lengths"
+
+let rec seq_zip_strict_list (seqs : 'a Seq.t list) : 'a list Seq.t =
+  match seqs with
+  | [] -> failwith "empty zip"
+  | [seq] -> seq |> Seq.map (fun x -> [x])
+  | seq :: seqs' ->
+    let seqs'_zip = seq_zip_strict_list seqs' in
+    seq_zip_strict seq seqs'_zip |> Seq.map (fun (x, xs) -> x :: xs)
+
+let seq_zip_strict_array (seqs : 'a Seq.t array) : 'a array Seq.t =
+  seqs |> Array.to_list |> seq_zip_strict_list |> Seq.map Array.of_list
 
 exception Dependent
 
@@ -34,7 +60,7 @@ let rec compose_arrows (hyps : EConstr.t list) (concl : EConstr.t) : EConstr.t =
   | hyp :: hyps' -> EConstr.mkProd (EConstr.anonR, hyp, EConstr.Vars.lift 1 (compose_arrows hyps' concl))
 
 let econstr_substl_opt (sigma : Evd.evar_map) (ts : EConstr.t option list) (c : EConstr.t) : EConstr.t =
-  assert (ts |> CList.for_all_i (fun t_i t -> c |> EConstr.Vars.noccurn sigma (1 + t_i) || Option.has_some t) 0);
+  (* assert (ts |> CList.for_all_i (fun t_i t -> c |> EConstr.Vars.noccurn sigma (1 + t_i) || Option.has_some t) 0); *)
   c |> EConstr.Vars.substl (ts |> List.map (Option.default EConstr.mkProp))
 
 let get_ref (env : Environ.env) (s : string) : EConstr.t =
@@ -55,6 +81,9 @@ let mk_eq_type (env : Environ.env) (typ : EConstr.t) (x : EConstr.t) (y : EConst
 
 let mk_eq_refl (env : Environ.env) (typ : EConstr.t) (x : EConstr.t) : EConstr.t =
   EConstr.mkApp (get_ref env "core.eq.refl", [|typ; x|])
+
+let mk_eq_trans (env : Environ.env) (typ : EConstr.t) (x : EConstr.t) (y : EConstr.t) (z : EConstr.t) (h_x_y : EConstr.t) (h_y_z : EConstr.t) : EConstr.t =
+  EConstr.mkApp (get_ref env "core.eq.trans", [|typ; x; y; z; h_x_y; h_y_z|])
 
 let mk_True_type (env : Environ.env) : EConstr.t =
   get_ref env "core.True.type"
@@ -104,6 +133,12 @@ let rec of_list_constr (env : Environ.env) (sigma : Evd.evar_map) (c : EConstr.t
 
 let mk_vector_type (env : Environ.env) (element_typ : EConstr.t) (len : EConstr.t) : EConstr.t =
   EConstr.mkApp (get_ref env "vcpu.vector.type", [|element_typ; len|])
+
+let is_vector_type (env : Environ.env) (sigma : Evd.evar_map) (typ : EConstr.t) : bool =
+  match EConstr.kind sigma typ with
+  | App (typ_head, [|_; _|]) when EConstr.eq_constr sigma typ_head (get_ref env "vcpu.vector.type") ->
+    true
+  | _ -> false
 
 let dest_vector_type (env : Environ.env) (sigma : Evd.evar_map) (typ : EConstr.t) : EConstr.t * EConstr.t =
   match EConstr.kind sigma typ with
@@ -158,12 +193,51 @@ let mk_circuit_eval_combine_relative (env : Environ.env) (n : EConstr.t) (m : EC
 let mk_circuit_combine_cong (env : Environ.env) (n : EConstr.t) (m : EConstr.t) (k : EConstr.t) (circuit_1 : EConstr.t) (circuit_1' : EConstr.t) (circuit_2 : EConstr.t) (circuit_2' : EConstr.t) (h_1 : EConstr.t) (h_2 : EConstr.t) : EConstr.t =
   EConstr.mkApp (get_ref env "vcpu.circuit.combine_cong", [|n; m; k; circuit_1; circuit_1'; circuit_2; circuit_2'; h_1; h_2|])
 
+let mk_circuit_comp_suffix (env : Environ.env) (n : EConstr.t) (m : EConstr.t) (k : EConstr.t) (circuit : EConstr.t)  : EConstr.t =
+  EConstr.mkApp (get_ref env "vcpu.circuit.comp_suffix", [|n; m; k; circuit|])
+
+let mk_circuit_wf_comp_suffix (env : Environ.env) (n : EConstr.t) (m : EConstr.t) (k : EConstr.t) (circuit : EConstr.t) (wf_circuit : EConstr.t) : EConstr.t =
+  EConstr.mkApp (get_ref env "vcpu.circuit.wf_comp_suffix", [|n; m; k; circuit; wf_circuit|])
+
+let mk_circuit_eval_comp_suffix (env : Environ.env) (n : EConstr.t) (m : EConstr.t) (k : EConstr.t) (circuit : EConstr.t) (wf_circuit : EConstr.t) (inputs : EConstr.t) (u : EConstr.t) (v : EConstr.t) (h_circuit : EConstr.t) : EConstr.t =
+  EConstr.mkApp (get_ref env "vcpu.circuit.eval_comp_suffix", [|n; m; k; circuit; wf_circuit; inputs; u; v; h_circuit|])
+
+let mk_circuit_comp_suffix_cong (env : Environ.env) (n : EConstr.t) (m : EConstr.t) (k : EConstr.t) (circuit : EConstr.t) (circuit' : EConstr.t) (h : EConstr.t) : EConstr.t =
+  EConstr.mkApp (get_ref env "vcpu.circuit.comp_suffix_cong", [|n; m; k; circuit; circuit'; h|])
+
+let mk_circuit_comp_prefix (env : Environ.env) (n : EConstr.t) (m : EConstr.t) (k : EConstr.t) (circuit : EConstr.t)  : EConstr.t =
+  EConstr.mkApp (get_ref env "vcpu.circuit.comp_prefix", [|n; m; k; circuit|])
+
+let mk_circuit_wf_comp_prefix (env : Environ.env) (n : EConstr.t) (m : EConstr.t) (k : EConstr.t) (circuit : EConstr.t) (wf_circuit : EConstr.t) : EConstr.t =
+  EConstr.mkApp (get_ref env "vcpu.circuit.wf_comp_prefix", [|n; m; k; circuit; wf_circuit|])
+
+let mk_circuit_eval_comp_prefix (env : Environ.env) (n : EConstr.t) (m : EConstr.t) (k : EConstr.t) (circuit : EConstr.t) (wf_circuit : EConstr.t) (inputs : EConstr.t) (u : EConstr.t) (v : EConstr.t) (h_circuit : EConstr.t) : EConstr.t =
+  EConstr.mkApp (get_ref env "vcpu.circuit.eval_comp_prefix", [|n; m; k; circuit; wf_circuit; inputs; u; v; h_circuit|])
+
+let mk_circuit_comp_prefix_cong (env : Environ.env) (n : EConstr.t) (m : EConstr.t) (k : EConstr.t) (circuit : EConstr.t) (circuit' : EConstr.t) (h : EConstr.t) : EConstr.t =
+  EConstr.mkApp (get_ref env "vcpu.circuit.comp_prefix_cong", [|n; m; k; circuit; circuit'; h|])
+
+let mk_circuit_comp_select (env : Environ.env) (n : EConstr.t) (m : EConstr.t) (k : EConstr.t) (l : EConstr.t) (circuit_1 : EConstr.t) (circuit_2 : EConstr.t) (circuit_3 : EConstr.t) : EConstr.t =
+  EConstr.mkApp (get_ref env "vcpu.circuit.comp_select", [|n; m; k; l; circuit_1; circuit_2; circuit_3|])
+
+let mk_circuit_wf_comp_select (env : Environ.env) (n : EConstr.t) (m : EConstr.t) (k : EConstr.t) (l : EConstr.t) (circuit_1 : EConstr.t) (circuit_2 : EConstr.t) (circuit_3 : EConstr.t) (wf_circuit_1 : EConstr.t) (wf_circuit_2 : EConstr.t) (wf_circuit_3 : EConstr.t) : EConstr.t =
+  EConstr.mkApp (get_ref env "vcpu.circuit.wf_comp_select", [|n; m; k; l; circuit_1; circuit_2; circuit_3; wf_circuit_1; wf_circuit_2; wf_circuit_3|])
+
+let mk_circuit_eval_comp_select_1 (env : Environ.env) (n : EConstr.t) (m : EConstr.t) (k : EConstr.t) (l : EConstr.t) (circuit_1 : EConstr.t) (circuit_2 : EConstr.t) (circuit_3 : EConstr.t) (wf_circuit_1 : EConstr.t) (wf_circuit_2 : EConstr.t) (wf_circuit_3 : EConstr.t) (inputs : EConstr.t) (u : EConstr.t) (v : EConstr.t) (w : EConstr.t) (h_circuit_1 : EConstr.t) (h_circuit_2 : EConstr.t) : EConstr.t =
+  EConstr.mkApp (get_ref env "vcpu.circuit.eval_comp_select_1", [|n; m; k; l; circuit_1; circuit_2; circuit_3; wf_circuit_1; wf_circuit_2; wf_circuit_3; inputs; u; v; w; h_circuit_1; h_circuit_2|])
+
+let mk_circuit_eval_comp_select_2 (env : Environ.env) (n : EConstr.t) (m : EConstr.t) (k : EConstr.t) (l : EConstr.t) (circuit_1 : EConstr.t) (circuit_2 : EConstr.t) (circuit_3 : EConstr.t) (wf_circuit_1 : EConstr.t) (wf_circuit_2 : EConstr.t) (wf_circuit_3 : EConstr.t) (inputs : EConstr.t) (u : EConstr.t) (v : EConstr.t) (w : EConstr.t) (h_circuit_1 : EConstr.t) (h_circuit_3 : EConstr.t) : EConstr.t =
+  EConstr.mkApp (get_ref env "vcpu.circuit.eval_comp_select_2", [|n; m; k; l; circuit_1; circuit_2; circuit_3; wf_circuit_1; wf_circuit_2; wf_circuit_3; inputs; u; v; w; h_circuit_1; h_circuit_3|])
+
+let mk_circuit_comp_select_cong (env : Environ.env) (n : EConstr.t) (m : EConstr.t) (k : EConstr.t) (l : EConstr.t) (circuit_1 : EConstr.t) (circuit_1' : EConstr.t) (circuit_2 : EConstr.t) (circuit_2' : EConstr.t) (circuit_3 : EConstr.t) (circuit_3' : EConstr.t) (wf_circuit_1' : EConstr.t) (h_1 : EConstr.t) (h_2 : EConstr.t) (h_3 : EConstr.t) : EConstr.t =
+  EConstr.mkApp (get_ref env "vcpu.circuit.comp_select_cong", [|n; m; k; l; circuit_1; circuit_1'; circuit_2; circuit_2'; circuit_3; circuit_3'; wf_circuit_1'; h_1; h_2; h_3|])
+
 type encoder = {
   encoder_len : EConstr.t;
   encoder_encode : EConstr.t;
 }
 
-let lift_encoder (n : int) (encoder : encoder) : encoder =
+let encoder_lift (n : int) (encoder : encoder) : encoder =
   {
     encoder_len = encoder.encoder_len |> EConstr.Vars.lift n;
     encoder_encode = encoder.encoder_encode |> EConstr.Vars.lift n;
@@ -273,7 +347,7 @@ let rec create_encoder (env : Environ.env) (sigma : Evd.evar_map) (context_encod
                     | None -> raise Static
                   )
               ) in
-            let constructor_type_lens =
+            let constructor_types_len =
               constructor_types_hyp_encoders
                 |> Array.map (fun constructor_type_hyp_encoders ->
                   List.fold_right (fun len_1 len_2 ->
@@ -281,7 +355,7 @@ let rec create_encoder (env : Environ.env) (sigma : Evd.evar_map) (context_encod
                   ) constructor_type_hyp_encoders (to_nat_constr env 0)
                 ) in
             let type_len =
-              constructor_type_lens
+              constructor_types_len
                 |> Array.to_list
                 |> reduce_right (fun len_1 len_2 ->
                   mk_nat_add env (to_nat_constr env 1) (mk_nat_add env len_1 len_2)
@@ -304,14 +378,14 @@ let rec create_encoder (env : Environ.env) (sigma : Evd.evar_map) (context_encod
                   ),
                   Constr.NoInvert,
                   EConstr.mkRel 1,
-                  constructor_types_hyp_encoders |> Array.mapi (fun constructor_1_i constructor_1_types_hyp_encoders ->
+                  constructor_types_hyp_encoders |> Array.mapi (fun constructor_1_i constructor_1_type_hyp_encoders ->
                     (
-                      constructor_1_types_hyp_encoders |> CArray.map_of_list (fun _ -> EConstr.anonR),
-                      (constructor_type_lens
+                      constructor_1_type_hyp_encoders |> CArray.map_of_list (fun _ -> EConstr.anonR),
+                      (constructor_types_len
                         |> Array.mapi (fun constructor_2_i constructor_2_type_len ->
-                          let constructor_1_types_hyp_encoders =
-                            constructor_1_types_hyp_encoders |> List.map (lift_encoder (1 + List.length constructor_1_types_hyp_encoders)) in
-                          let constructor_2_type_len = constructor_2_type_len |> EConstr.Vars.lift (1 + List.length constructor_1_types_hyp_encoders) in
+                          let constructor_1_type_hyp_encoders =
+                            constructor_1_type_hyp_encoders |> List.map (encoder_lift (1 + List.length constructor_1_type_hyp_encoders)) in
+                          let constructor_2_type_len = constructor_2_type_len |> EConstr.Vars.lift (1 + List.length constructor_1_type_hyp_encoders) in
                           if constructor_2_i = constructor_1_i then
                             List.fold_right
                               (fun encoder_1 encoder_2 ->
@@ -324,16 +398,16 @@ let rec create_encoder (env : Environ.env) (sigma : Evd.evar_map) (context_encod
                                       encoder_1.encoder_len
                                       encoder_2.encoder_len
                                       encoder_1.encoder_encode
-                                      encoder_2.encoder_encode
+                                      encoder_2.encoder_encode;
                                 }
                               )
-                              (constructor_1_types_hyp_encoders |> List.mapi (fun i constructor_1_types_hyp_encoder ->
+                              (constructor_1_type_hyp_encoders |> List.mapi (fun arg_i constructor_1_type_hyp_encoder ->
                                 {
-                                  encoder_len = constructor_1_types_hyp_encoder.encoder_len;
+                                  encoder_len = constructor_1_type_hyp_encoder.encoder_len;
                                   encoder_encode =
                                     EConstr.mkApp (
-                                      constructor_1_types_hyp_encoder.encoder_encode,
-                                      [|EConstr.mkRel (List.length constructor_1_types_hyp_encoders - i)|]
+                                      constructor_1_type_hyp_encoder.encoder_encode,
+                                      [|EConstr.mkRel (List.length constructor_1_type_hyp_encoders - arg_i)|]
                                     );
                                 }
                               ))
@@ -349,7 +423,7 @@ let rec create_encoder (env : Environ.env) (sigma : Evd.evar_map) (context_encod
                             }
                         )
                         |> Array.to_list
-                        |> reduce_right_i (fun i encoder_1 encoder_2 ->
+                        |> reduce_right_i (fun constructor_2_i encoder_1 encoder_2 ->
                           {
                             encoder_len =
                               mk_nat_add env (to_nat_constr env 1) (mk_nat_add env encoder_1.encoder_len encoder_2.encoder_len);
@@ -358,7 +432,7 @@ let rec create_encoder (env : Environ.env) (sigma : Evd.evar_map) (context_encod
                                 (mk_bool_type env)
                                 (to_nat_constr env 1)
                                 (mk_nat_add env encoder_1.encoder_len encoder_2.encoder_len)
-                                (to_vector_constr env (mk_bool_type env) [to_bool_constr env (i = constructor_1_i)])
+                                (to_vector_constr env (mk_bool_type env) [to_bool_constr env (constructor_2_i = constructor_1_i)])
                                 (mk_vector_app env
                                   (mk_bool_type env)
                                   encoder_1.encoder_len
@@ -410,7 +484,7 @@ let entry_derive_encoder (input_type_constr_expr : Constrexpr.constr_expr) (outp
       None ::
       None ::
       Some {encoder_len = EConstr.mkRel 2; encoder_encode = EConstr.mkRel 1} ::
-      (encoders |> List.map (Option.map (lift_encoder 3)))
+      (encoders |> List.map (Option.map (encoder_lift 3)))
     ) [] input_type_type_hyps in
   let app_input_type =
     EConstr.mkApp (
@@ -542,14 +616,14 @@ let rec enumerate_reprs (env : Environ.env) (sigma : Evd.evar_map) (context_enco
           None ::
           None ::
           Some {encoder_len = EConstr.mkRel 2; encoder_encode = EConstr.mkRel 1} ::
-          (context_encoders |> List.map (Option.map (lift_encoder 3)))
+          (context_encoders |> List.map (Option.map (encoder_lift 3)))
         )
         (type_2 |> EConstr.Vars.liftn 3 2 |> EConstr.Vars.subst1 (EConstr.mkRel 3))
         |> List.map (fun type_2_repr -> ReprFunctional (ReprTransformed, type_2_repr))) @
       (enumerate_reprs
         (env |> EConstr.push_rel (Context.Rel.Declaration.LocalAssum (EConstr.anonR, type_1)))
         sigma
-        (None :: (context_encoders |> List.map (Option.map (lift_encoder 1))))
+        (None :: (context_encoders |> List.map (Option.map (encoder_lift 1))))
         type_2
         |> List.map (fun type_2_repr -> ReprFunctional (ReprRaw, type_2_repr)))
     else if
@@ -575,7 +649,7 @@ type compilation = {
   compilation_eq_circuit_erased : EConstr.t;
 }
 
-let lift_compilation (n : int) (compilation : compilation) : compilation =
+let compilation_lift (n : int) (compilation : compilation) : compilation =
   {
     compilation_orig = compilation.compilation_orig |> EConstr.Vars.lift n;
     compilation_circuit = compilation.compilation_circuit |> EConstr.Vars.lift n;
@@ -583,6 +657,36 @@ let lift_compilation (n : int) (compilation : compilation) : compilation =
     compilation_eval_circuit = compilation.compilation_eval_circuit |> EConstr.Vars.lift n;
     compilation_circuit_erased = compilation.compilation_circuit_erased |> EConstr.Vars.lift n;
     compilation_eq_circuit_erased = compilation.compilation_eq_circuit_erased |> EConstr.Vars.lift n;
+  }
+
+let compilation_liftn (n : int) (m : int) (compilation : compilation) : compilation =
+  {
+    compilation_orig = compilation.compilation_orig |> EConstr.Vars.liftn n m;
+    compilation_circuit = compilation.compilation_circuit |> EConstr.Vars.liftn n m;
+    compilation_wf_circuit = compilation.compilation_wf_circuit |> EConstr.Vars.liftn n m;
+    compilation_eval_circuit = compilation.compilation_eval_circuit |> EConstr.Vars.liftn n m;
+    compilation_circuit_erased = compilation.compilation_circuit_erased |> EConstr.Vars.liftn n m;
+    compilation_eq_circuit_erased = compilation.compilation_eq_circuit_erased |> EConstr.Vars.liftn n m;
+  }
+
+let compilation_substl (l : EConstr.t list) (compilation : compilation) : compilation =
+  {
+    compilation_orig = compilation.compilation_orig |> EConstr.Vars.substl l;
+    compilation_circuit = compilation.compilation_circuit |> EConstr.Vars.substl l;
+    compilation_wf_circuit = compilation.compilation_wf_circuit |> EConstr.Vars.substl l;
+    compilation_eval_circuit = compilation.compilation_eval_circuit |> EConstr.Vars.substl l;
+    compilation_circuit_erased = compilation.compilation_circuit_erased |> EConstr.Vars.substl l;
+    compilation_eq_circuit_erased = compilation.compilation_eq_circuit_erased |> EConstr.Vars.substl l;
+  }
+
+let compilation_substl_opt (sigma : Evd.evar_map) (l : EConstr.t option list) (compilation : compilation) : compilation =
+  {
+    compilation_orig = compilation.compilation_orig |> econstr_substl_opt sigma l;
+    compilation_circuit = compilation.compilation_circuit |> econstr_substl_opt sigma l;
+    compilation_wf_circuit = compilation.compilation_wf_circuit |> econstr_substl_opt sigma l;
+    compilation_eval_circuit = compilation.compilation_eval_circuit |> econstr_substl_opt sigma l;
+    compilation_circuit_erased = compilation.compilation_circuit_erased |> econstr_substl_opt sigma l;
+    compilation_eq_circuit_erased = compilation.compilation_eq_circuit_erased |> econstr_substl_opt sigma l;
   }
 
 let compilation_type_to_context (annot : Names.Name.t EConstr.binder_annot) (compilation : compilation) : EConstr.rel_context =
@@ -671,8 +775,8 @@ let rec get_compilation_type (env : Environ.env) (sigma : Evd.evar_map) (context
           get_compilation_type
             (EConstr.push_rel (Context.Rel.Declaration.LocalAssum (EConstr.anonR, type_1)) env)
             sigma
-            (None :: (context_encoders |> List.map (Option.map (lift_encoder 1))))
-            (input_encoder |> lift_encoder 1)
+            (None :: (context_encoders |> List.map (Option.map (encoder_lift 1))))
+            (input_encoder |> encoder_lift 1)
             type_2
             type_2_repr in
         {
@@ -764,9 +868,9 @@ let rec get_compilation_type (env : Environ.env) (sigma : Evd.evar_map) (context
                 None ::
                 None ::
                 Some {encoder_len = EConstr.mkRel 2; encoder_encode = EConstr.mkRel 1} ::
-                (context_encoders |> List.map (Option.map (lift_encoder 3)))
+                (context_encoders |> List.map (Option.map (encoder_lift 3)))
               )
-              (input_encoder |> lift_encoder 3)
+              (input_encoder |> encoder_lift 3)
               (type_2 |> EConstr.Vars.liftn 3 2 |> EConstr.Vars.subst1 (EConstr.mkRel 3))
               type_2_repr in
           {
@@ -852,10 +956,10 @@ let rec get_compilation_type (env : Environ.env) (sigma : Evd.evar_map) (context
         then
           let type_1_compilation_type =
             get_compilation_type env sigma context_encoders input_encoder type_1 type_1_repr in
-          let type_1_context = type_1_compilation_type |> compilation_type_to_context type_annot in
+          let type_1_ctx = type_1_compilation_type |> compilation_type_to_context type_annot in
           let type_2_compilation_type =
             get_compilation_type
-              (env |> EConstr.push_rel_context type_1_context)
+              (env |> EConstr.push_rel_context type_1_ctx)
               sigma
               (
                 None ::
@@ -864,9 +968,9 @@ let rec get_compilation_type (env : Environ.env) (sigma : Evd.evar_map) (context
                 None ::
                 None ::
                 None ::
-                (context_encoders |> List.map (Option.map (lift_encoder 6)))
+                (context_encoders |> List.map (Option.map (encoder_lift 6)))
               )
-              (input_encoder |> lift_encoder 6)
+              (input_encoder |> encoder_lift 6)
               (type_2 |> EConstr.Vars.liftn 6 2 |> EConstr.Vars.subst1 (EConstr.mkRel 6))
               type_2_repr in
           {
@@ -882,7 +986,7 @@ let rec get_compilation_type (env : Environ.env) (sigma : Evd.evar_map) (context
                     EConstr.mkRel 5;
                     EConstr.mkRel 6;
                   ])
-                (type_1_context |> EConstr.Vars.lift_rel_context 0);
+                (type_1_ctx |> EConstr.Vars.lift_rel_context 0);
             compilation_circuit =
               EConstr.it_mkProd_or_LetIn
                 (type_2_compilation_type.compilation_circuit
@@ -896,7 +1000,7 @@ let rec get_compilation_type (env : Environ.env) (sigma : Evd.evar_map) (context
                     EConstr.mkRel 5;
                     EConstr.mkRel 6;
                   ])
-                (type_1_context |> EConstr.Vars.lift_rel_context 1);
+                (type_1_ctx |> EConstr.Vars.lift_rel_context 1);
             compilation_wf_circuit =
               EConstr.it_mkProd_or_LetIn
                 (type_2_compilation_type.compilation_wf_circuit
@@ -911,7 +1015,7 @@ let rec get_compilation_type (env : Environ.env) (sigma : Evd.evar_map) (context
                     EConstr.mkRel 5;
                     EConstr.mkRel 6;
                   ])
-                (type_1_context |> EConstr.Vars.lift_rel_context 2);
+                (type_1_ctx |> EConstr.Vars.lift_rel_context 2);
             compilation_eval_circuit =
               EConstr.it_mkProd_or_LetIn
                 (type_2_compilation_type.compilation_eval_circuit
@@ -927,7 +1031,7 @@ let rec get_compilation_type (env : Environ.env) (sigma : Evd.evar_map) (context
                     EConstr.mkRel 5;
                     EConstr.mkRel 6;
                   ])
-                (type_1_context |> EConstr.Vars.lift_rel_context 3);
+                (type_1_ctx |> EConstr.Vars.lift_rel_context 3);
             compilation_circuit_erased =
               EConstr.mkProd (EConstr.anonR,
                 type_1_compilation_type.compilation_circuit_erased
@@ -970,7 +1074,7 @@ let rec get_compilation_type (env : Environ.env) (sigma : Evd.evar_map) (context
                     EConstr.mkRel 5;
                     EConstr.mkRel 6;
                   ])
-                (type_1_context |> EConstr.Vars.lift_rel_context 5);
+                (type_1_ctx |> EConstr.Vars.lift_rel_context 5);
           }
         else
           assert false
@@ -1051,6 +1155,742 @@ let mk_compilation_combine (env : Environ.env) (orig : EConstr.t) (n : EConstr.t
         compilation_2.compilation_eq_circuit_erased;
   }
 
+let mk_compilation_comp_prefix (env : Environ.env) (orig : EConstr.t) (n : EConstr.t) (m : EConstr.t) (k : EConstr.t) (compilation : compilation) (inputs : EConstr.t) (u : EConstr.t) (v : EConstr.t) : compilation =
+  {
+    compilation_orig = orig;
+    compilation_circuit =
+      mk_circuit_comp_prefix env
+        n
+        m
+        k
+        compilation.compilation_circuit;
+    compilation_wf_circuit =
+      mk_circuit_wf_comp_prefix env
+        n
+        m
+        k
+        compilation.compilation_circuit
+        compilation.compilation_wf_circuit;
+    compilation_eval_circuit =
+      mk_circuit_eval_comp_prefix env
+        n
+        m
+        k
+        compilation.compilation_circuit
+        compilation.compilation_wf_circuit
+        inputs
+        u
+        v
+        compilation.compilation_eval_circuit;
+    compilation_circuit_erased =
+      mk_circuit_comp_prefix env
+        n
+        m
+        k
+        compilation.compilation_circuit_erased;
+    compilation_eq_circuit_erased =
+      mk_circuit_comp_prefix_cong env
+        n
+        m
+        k
+        compilation.compilation_circuit_erased
+        compilation.compilation_circuit
+        compilation.compilation_eq_circuit_erased;
+  }
+
+let mk_compilation_comp_suffix (env : Environ.env) (orig : EConstr.t) (n : EConstr.t) (m : EConstr.t) (k : EConstr.t) (compilation : compilation) (inputs : EConstr.t) (u : EConstr.t) (v : EConstr.t) : compilation =
+  {
+    compilation_orig = orig;
+    compilation_circuit =
+      mk_circuit_comp_suffix env
+        n
+        m
+        k
+        compilation.compilation_circuit;
+    compilation_wf_circuit =
+      mk_circuit_wf_comp_suffix env
+        n
+        m
+        k
+        compilation.compilation_circuit
+        compilation.compilation_wf_circuit;
+    compilation_eval_circuit =
+      mk_circuit_eval_comp_suffix env
+        n
+        m
+        k
+        compilation.compilation_circuit
+        compilation.compilation_wf_circuit
+        inputs
+        u
+        v
+        compilation.compilation_eval_circuit;
+    compilation_circuit_erased =
+      mk_circuit_comp_suffix env
+        n
+        m
+        k
+        compilation.compilation_circuit_erased;
+    compilation_eq_circuit_erased =
+      mk_circuit_comp_suffix_cong env
+        n
+        m
+        k
+        compilation.compilation_circuit_erased
+        compilation.compilation_circuit
+        compilation.compilation_eq_circuit_erased;
+  }
+
+let mk_compilation_comp_select_1 (env : Environ.env) (sigma : Evd.evar_map) (n : EConstr.t) (m : EConstr.t) (k : EConstr.t) (l : EConstr.t) (compilation_1 : compilation) (compilations_2 : EConstr.rel_context -> compilation -> compilation Seq.t) (compilations_3 : EConstr.rel_context -> compilation -> compilation Seq.t) (inputs : EConstr.t) (u : EConstr.t) (v : EConstr.t) (w : EConstr.t) : compilation Seq.t =
+  compilations_2
+  [
+    Context.Rel.Declaration.LocalAssum (EConstr.anonR,
+      mk_eq_type env
+        (mk_vector_type env (mk_bool_type env) (m |> EConstr.Vars.lift 2))
+        (mk_circuit_eval env
+          (n |> EConstr.Vars.lift 2)
+          (m |> EConstr.Vars.lift 2)
+          (EConstr.mkRel 2)
+          (inputs |> EConstr.Vars.lift 2))
+        (u |> EConstr.Vars.lift 2)
+    );
+    Context.Rel.Declaration.LocalAssum (EConstr.anonR,
+      mk_circuit_wf env
+        (n |> EConstr.Vars.lift 1)
+        (m |> EConstr.Vars.lift 1)
+        (EConstr.mkRel 1)
+    );
+    Context.Rel.Declaration.LocalAssum (EConstr.anonR,
+      mk_circuit_type env
+        n
+        m
+    );
+  ]
+  {
+    compilation_orig = mk_unit_tt env;
+    compilation_circuit = EConstr.mkRel 3;
+    compilation_wf_circuit = EConstr.mkRel 2;
+    compilation_eval_circuit = EConstr.mkRel 1;
+    compilation_circuit_erased = EConstr.mkRel 3;
+    compilation_eq_circuit_erased =
+      mk_eq_refl env
+        (mk_circuit_type env
+          (n |> EConstr.Vars.lift 3)
+          (m |> EConstr.Vars.lift 3))
+        (EConstr.mkRel 3);
+  }
+    |> Seq.flat_map (fun compilation_2_res ->
+      compilations_3
+      [
+        Context.Rel.Declaration.LocalAssum (EConstr.anonR,
+          mk_circuit_wf env
+            (n |> EConstr.Vars.lift 1)
+            (k |> EConstr.Vars.lift 2)
+            (EConstr.mkRel 1)
+        );
+        Context.Rel.Declaration.LocalAssum (EConstr.anonR,
+          mk_circuit_type env
+            n
+            k
+        );
+      ]
+      {
+        compilation_orig = mk_unit_tt env;
+        compilation_circuit = EConstr.mkRel 2;
+        compilation_wf_circuit = EConstr.mkRel 1;
+        compilation_eval_circuit = mk_True_I env;
+        compilation_circuit_erased = EConstr.mkRel 2;
+        compilation_eq_circuit_erased =
+          mk_eq_refl env
+            (mk_circuit_type env
+              (n |> EConstr.Vars.lift 2)
+              (k |> EConstr.Vars.lift 2))
+            (EConstr.mkRel 2);
+      }
+        |> Seq.flat_map (fun compilation_3_res ->
+          Seq.return {
+            compilation_orig =
+              compilation_2_res.compilation_orig
+                |> EConstr.Vars.liftn 0 4
+                |> econstr_substl_opt sigma [None; None; None];
+            compilation_circuit =
+              mk_circuit_comp_select env
+                n
+                m
+                k
+                l
+                compilation_1.compilation_circuit
+                (EConstr.mkLambda (EConstr.anonR,
+                  mk_circuit_type env
+                    n
+                    m,
+                  compilation_2_res.compilation_circuit
+                    |> EConstr.Vars.liftn 1 4
+                    |> econstr_substl_opt sigma [None; None; Some (EConstr.mkRel 1)]
+                ))
+                (EConstr.mkLambda (EConstr.anonR,
+                  mk_circuit_type env
+                    n
+                    k,
+                  compilation_3_res.compilation_circuit
+                    |> EConstr.Vars.liftn 1 3
+                    |> econstr_substl_opt sigma [None; Some (EConstr.mkRel 1)]
+                ));
+            compilation_wf_circuit =
+              mk_circuit_wf_comp_select env
+                n
+                m
+                k
+                l
+                compilation_1.compilation_circuit
+                (EConstr.mkLambda (EConstr.anonR,
+                  mk_circuit_type env
+                    n
+                    m,
+                  compilation_2_res.compilation_circuit
+                    |> EConstr.Vars.liftn 1 4
+                    |> econstr_substl_opt sigma [None; None; Some (EConstr.mkRel 1)]
+                ))
+                (EConstr.mkLambda (EConstr.anonR,
+                  mk_circuit_type env
+                    n
+                    k,
+                  compilation_3_res.compilation_circuit
+                    |> EConstr.Vars.liftn 1 3
+                    |> econstr_substl_opt sigma [None; Some (EConstr.mkRel 1)]
+                ))
+                compilation_1.compilation_wf_circuit
+                (EConstr.mkLambda (EConstr.anonR,
+                  mk_circuit_type env
+                    n
+                    m,
+                  EConstr.mkLambda (EConstr.anonR,
+                    mk_circuit_wf env
+                      (n |> EConstr.Vars.lift 1)
+                      (m |> EConstr.Vars.lift 1)
+                      (EConstr.mkRel 1),
+                    compilation_2_res.compilation_wf_circuit
+                      |> EConstr.Vars.liftn 2 4
+                      |> econstr_substl_opt sigma [None; Some (EConstr.mkRel 1); Some (EConstr.mkRel 2)]
+                  )
+                ))
+                (EConstr.mkLambda (EConstr.anonR,
+                  mk_circuit_type env
+                    n
+                    k,
+                  EConstr.mkLambda (EConstr.anonR,
+                    mk_circuit_wf env
+                      (n |> EConstr.Vars.lift 1)
+                      (k |> EConstr.Vars.lift 1)
+                      (EConstr.mkRel 1),
+                    compilation_3_res.compilation_wf_circuit
+                      |> EConstr.Vars.liftn 2 3
+                      |> econstr_substl_opt sigma [Some (EConstr.mkRel 1); Some (EConstr.mkRel 2)]
+                  )
+                ));
+            compilation_eval_circuit =
+              mk_circuit_eval_comp_select_1 env
+                n
+                m
+                k
+                l
+                compilation_1.compilation_circuit
+                (EConstr.mkLambda (EConstr.anonR,
+                  mk_circuit_type env
+                    n
+                    m,
+                  compilation_2_res.compilation_circuit
+                    |> EConstr.Vars.liftn 1 4
+                    |> econstr_substl_opt sigma [None; None; Some (EConstr.mkRel 1)]
+                ))
+                (EConstr.mkLambda (EConstr.anonR,
+                  mk_circuit_type env
+                    n
+                    k,
+                  compilation_3_res.compilation_circuit
+                    |> EConstr.Vars.liftn 1 3
+                    |> econstr_substl_opt sigma [None; Some (EConstr.mkRel 1)]
+                ))
+                compilation_1.compilation_wf_circuit
+                (EConstr.mkLambda (EConstr.anonR,
+                  mk_circuit_type env
+                    n
+                    m,
+                  EConstr.mkLambda (EConstr.anonR,
+                    mk_circuit_wf env
+                      (n |> EConstr.Vars.lift 1)
+                      (m |> EConstr.Vars.lift 1)
+                      (EConstr.mkRel 1),
+                    compilation_2_res.compilation_wf_circuit
+                      |> EConstr.Vars.liftn 2 4
+                      |> econstr_substl_opt sigma [None; Some (EConstr.mkRel 1); Some (EConstr.mkRel 2)]
+                  )
+                ))
+                (EConstr.mkLambda (EConstr.anonR,
+                  mk_circuit_type env
+                    n
+                    k,
+                  EConstr.mkLambda (EConstr.anonR,
+                    mk_circuit_wf env
+                      (n |> EConstr.Vars.lift 1)
+                      (k |> EConstr.Vars.lift 1)
+                      (EConstr.mkRel 1),
+                    compilation_3_res.compilation_wf_circuit
+                      |> EConstr.Vars.liftn 2 3
+                      |> econstr_substl_opt sigma [Some (EConstr.mkRel 1); Some (EConstr.mkRel 2)]
+                  )
+                ))
+                inputs
+                u
+                v
+                w
+                compilation_1.compilation_eval_circuit
+                (EConstr.mkLambda (EConstr.anonR,
+                  mk_circuit_type env
+                    n
+                    m,
+                  EConstr.mkLambda (EConstr.anonR,
+                    mk_circuit_wf env
+                      (n |> EConstr.Vars.lift 1)
+                      (m |> EConstr.Vars.lift 1)
+                      (EConstr.mkRel 1),
+                    EConstr.mkLambda (EConstr.anonR,
+                      mk_eq_type env
+                        (mk_vector_type env (mk_bool_type env) (m |> EConstr.Vars.lift 2))
+                        (mk_circuit_eval env
+                          (n |> EConstr.Vars.lift 2)
+                          (m |> EConstr.Vars.lift 2)
+                          (EConstr.mkRel 2)
+                          (inputs |> EConstr.Vars.lift 2))
+                        (u |> EConstr.Vars.lift 2),
+                      compilation_2_res.compilation_eval_circuit
+                        |> EConstr.Vars.liftn 3 4
+                        |> econstr_substl_opt sigma [Some (EConstr.mkRel 1); Some (EConstr.mkRel 2); Some (EConstr.mkRel 3)]
+                    )
+                  )
+                ));
+            compilation_circuit_erased =
+              mk_circuit_comp_select env
+                n
+                m
+                k
+                l
+                compilation_1.compilation_circuit_erased
+                (EConstr.mkLambda (EConstr.anonR,
+                  mk_circuit_type env
+                    n
+                    m,
+                  compilation_2_res.compilation_circuit_erased
+                    |> EConstr.Vars.liftn 1 4
+                    |> econstr_substl_opt sigma [None; None; Some (EConstr.mkRel 1)]
+                ))
+                (EConstr.mkLambda (EConstr.anonR,
+                  mk_circuit_type env
+                    n
+                    k,
+                  compilation_3_res.compilation_circuit_erased
+                    |> EConstr.Vars.liftn 1 3
+                    |> econstr_substl_opt sigma [None; Some (EConstr.mkRel 1)]
+                ));
+            compilation_eq_circuit_erased =
+              mk_circuit_comp_select_cong env
+                n
+                m
+                k
+                l
+                compilation_1.compilation_circuit_erased
+                compilation_1.compilation_circuit
+                (EConstr.mkLambda (EConstr.anonR,
+                  mk_circuit_type env
+                    n
+                    m,
+                  compilation_2_res.compilation_circuit_erased
+                    |> EConstr.Vars.liftn 1 4
+                    |> econstr_substl_opt sigma [None; None; Some (EConstr.mkRel 1)]
+                ))
+                (EConstr.mkLambda (EConstr.anonR,
+                  mk_circuit_type env
+                    n
+                    m,
+                  compilation_2_res.compilation_circuit
+                    |> EConstr.Vars.liftn 1 4
+                    |> econstr_substl_opt sigma [None; None; Some (EConstr.mkRel 1)]
+                ))
+                (EConstr.mkLambda (EConstr.anonR,
+                  mk_circuit_type env
+                    n
+                    k,
+                  compilation_3_res.compilation_circuit_erased
+                    |> EConstr.Vars.liftn 1 3
+                    |> econstr_substl_opt sigma [None; Some (EConstr.mkRel 1)]
+                ))
+                (EConstr.mkLambda (EConstr.anonR,
+                  mk_circuit_type env
+                    n
+                    k,
+                  compilation_3_res.compilation_circuit
+                    |> EConstr.Vars.liftn 1 3
+                    |> econstr_substl_opt sigma [None; Some (EConstr.mkRel 1)]
+                ))
+                compilation_1.compilation_wf_circuit
+                compilation_1.compilation_eq_circuit_erased
+                (EConstr.mkLambda (EConstr.anonR,
+                  mk_circuit_type env
+                    n
+                    m,
+                  EConstr.mkLambda (EConstr.anonR,
+                    mk_circuit_wf env
+                      (n |> EConstr.Vars.lift 1)
+                      (m |> EConstr.Vars.lift 1)
+                      (EConstr.mkRel 1),
+                    compilation_2_res.compilation_eq_circuit_erased
+                      |> EConstr.Vars.liftn 2 4
+                      |> econstr_substl_opt sigma [None; Some (EConstr.mkRel 1); Some (EConstr.mkRel 2)]
+                  )
+                ))
+                (EConstr.mkLambda (EConstr.anonR,
+                  mk_circuit_type env
+                    n
+                    k,
+                  EConstr.mkLambda (EConstr.anonR,
+                    mk_circuit_wf env
+                      (n |> EConstr.Vars.lift 1)
+                      (k |> EConstr.Vars.lift 1)
+                      (EConstr.mkRel 1),
+                    compilation_3_res.compilation_eq_circuit_erased
+                      |> EConstr.Vars.liftn 2 3
+                      |> econstr_substl_opt sigma [Some (EConstr.mkRel 1); Some (EConstr.mkRel 2)]
+                  )
+                ));
+          }
+        )
+    )
+
+let mk_compilation_comp_select_2 (env : Environ.env) (sigma : Evd.evar_map) (n : EConstr.t) (m : EConstr.t) (k : EConstr.t) (l : EConstr.t) (compilation_1 : compilation) (compilations_2 : EConstr.rel_context -> compilation -> compilation Seq.t) (compilations_3 : EConstr.rel_context -> compilation -> compilation Seq.t) (inputs : EConstr.t) (u : EConstr.t) (v : EConstr.t) (w : EConstr.t) : compilation Seq.t =
+  compilations_2
+  [
+    Context.Rel.Declaration.LocalAssum (EConstr.anonR,
+      mk_circuit_wf env
+        (n |> EConstr.Vars.lift 1)
+        (m |> EConstr.Vars.lift 2)
+        (EConstr.mkRel 1)
+    );
+    Context.Rel.Declaration.LocalAssum (EConstr.anonR,
+      mk_circuit_type env
+        n
+        m
+    );
+  ]
+  {
+    compilation_orig = mk_unit_tt env;
+    compilation_circuit = EConstr.mkRel 2;
+    compilation_wf_circuit = EConstr.mkRel 1;
+    compilation_eval_circuit = mk_True_I env;
+    compilation_circuit_erased = EConstr.mkRel 2;
+    compilation_eq_circuit_erased =
+      mk_eq_refl env
+        (mk_circuit_type env
+          (n |> EConstr.Vars.lift 2)
+          (m |> EConstr.Vars.lift 2))
+        (EConstr.mkRel 2);
+  }
+    |> Seq.flat_map (fun compilation_2_res ->
+      compilations_3
+      [
+        Context.Rel.Declaration.LocalAssum (EConstr.anonR,
+          mk_eq_type env
+            (mk_vector_type env (mk_bool_type env) (k |> EConstr.Vars.lift 2))
+            (mk_circuit_eval env
+              (n |> EConstr.Vars.lift 2)
+              (k |> EConstr.Vars.lift 2)
+              (EConstr.mkRel 2)
+              (inputs |> EConstr.Vars.lift 2))
+            (v |> EConstr.Vars.lift 2)
+        );
+        Context.Rel.Declaration.LocalAssum (EConstr.anonR,
+          mk_circuit_wf env
+            (n |> EConstr.Vars.lift 1)
+            (k |> EConstr.Vars.lift 1)
+            (EConstr.mkRel 1)
+        );
+        Context.Rel.Declaration.LocalAssum (EConstr.anonR,
+          mk_circuit_type env
+            n
+            k
+        );
+      ]
+      {
+        compilation_orig = mk_unit_tt env;
+        compilation_circuit = EConstr.mkRel 3;
+        compilation_wf_circuit = EConstr.mkRel 2;
+        compilation_eval_circuit = EConstr.mkRel 1;
+        compilation_circuit_erased = EConstr.mkRel 3;
+        compilation_eq_circuit_erased =
+          mk_eq_refl env
+            (mk_circuit_type env
+              (n |> EConstr.Vars.lift 3)
+              (k |> EConstr.Vars.lift 3))
+            (EConstr.mkRel 3);
+      }
+        |> Seq.flat_map (fun compilation_3_res ->
+          Seq.return {
+            compilation_orig =
+              compilation_3_res.compilation_orig
+                |> EConstr.Vars.liftn 0 4
+                |> econstr_substl_opt sigma [None; None; None];
+            compilation_circuit =
+              mk_circuit_comp_select env
+                n
+                m
+                k
+                l
+                compilation_1.compilation_circuit
+                (EConstr.mkLambda (EConstr.anonR,
+                  mk_circuit_type env
+                    n
+                    m,
+                  compilation_2_res.compilation_circuit
+                    |> EConstr.Vars.liftn 1 3
+                    |> econstr_substl_opt sigma [None; Some (EConstr.mkRel 1)]
+                ))
+                (EConstr.mkLambda (EConstr.anonR,
+                  mk_circuit_type env
+                    n
+                    k,
+                  compilation_3_res.compilation_circuit
+                    |> EConstr.Vars.liftn 1 4
+                    |> econstr_substl_opt sigma [None; None; Some (EConstr.mkRel 1)]
+                ));
+            compilation_wf_circuit =
+              mk_circuit_wf_comp_select env
+                n
+                m
+                k
+                l
+                compilation_1.compilation_circuit
+                (EConstr.mkLambda (EConstr.anonR,
+                  mk_circuit_type env
+                    n
+                    m,
+                  compilation_2_res.compilation_circuit
+                    |> EConstr.Vars.liftn 1 3
+                    |> econstr_substl_opt sigma [None; Some (EConstr.mkRel 1)]
+                ))
+                (EConstr.mkLambda (EConstr.anonR,
+                  mk_circuit_type env
+                    n
+                    k,
+                  compilation_3_res.compilation_circuit
+                    |> EConstr.Vars.liftn 1 4
+                    |> econstr_substl_opt sigma [None; None; Some (EConstr.mkRel 1)]
+                ))
+                compilation_1.compilation_wf_circuit
+                (EConstr.mkLambda (EConstr.anonR,
+                  mk_circuit_type env
+                    n
+                    m,
+                  EConstr.mkLambda (EConstr.anonR,
+                    mk_circuit_wf env
+                      (n |> EConstr.Vars.lift 1)
+                      (m |> EConstr.Vars.lift 1)
+                      (EConstr.mkRel 1),
+                    compilation_2_res.compilation_wf_circuit
+                      |> EConstr.Vars.liftn 2 3
+                      |> econstr_substl_opt sigma [Some (EConstr.mkRel 1); Some (EConstr.mkRel 2)]
+                  )
+                ))
+                (EConstr.mkLambda (EConstr.anonR,
+                  mk_circuit_type env
+                    n
+                    k,
+                  EConstr.mkLambda (EConstr.anonR,
+                    mk_circuit_wf env
+                      (n |> EConstr.Vars.lift 1)
+                      (k |> EConstr.Vars.lift 1)
+                      (EConstr.mkRel 1),
+                    compilation_3_res.compilation_wf_circuit
+                      |> EConstr.Vars.liftn 2 4
+                      |> econstr_substl_opt sigma [None; Some (EConstr.mkRel 1); Some (EConstr.mkRel 2)]
+                  )
+                ));
+            compilation_eval_circuit =
+              mk_circuit_eval_comp_select_2 env
+                n
+                m
+                k
+                l
+                compilation_1.compilation_circuit
+                (EConstr.mkLambda (EConstr.anonR,
+                  mk_circuit_type env
+                    n
+                    m,
+                  compilation_2_res.compilation_circuit
+                    |> EConstr.Vars.liftn 1 3
+                    |> econstr_substl_opt sigma [None; Some (EConstr.mkRel 1)]
+                ))
+                (EConstr.mkLambda (EConstr.anonR,
+                  mk_circuit_type env
+                    n
+                    k,
+                  compilation_3_res.compilation_circuit
+                    |> EConstr.Vars.liftn 1 4
+                    |> econstr_substl_opt sigma [None; None; Some (EConstr.mkRel 1)]
+                ))
+                compilation_1.compilation_wf_circuit
+                (EConstr.mkLambda (EConstr.anonR,
+                  mk_circuit_type env
+                    n
+                    m,
+                  EConstr.mkLambda (EConstr.anonR,
+                    mk_circuit_wf env
+                      (n |> EConstr.Vars.lift 1)
+                      (m |> EConstr.Vars.lift 1)
+                      (EConstr.mkRel 1),
+                    compilation_2_res.compilation_wf_circuit
+                      |> EConstr.Vars.liftn 2 3
+                      |> econstr_substl_opt sigma [Some (EConstr.mkRel 1); Some (EConstr.mkRel 2)]
+                  )
+                ))
+                (EConstr.mkLambda (EConstr.anonR,
+                  mk_circuit_type env
+                    n
+                    k,
+                  EConstr.mkLambda (EConstr.anonR,
+                    mk_circuit_wf env
+                      (n |> EConstr.Vars.lift 1)
+                      (k |> EConstr.Vars.lift 1)
+                      (EConstr.mkRel 1),
+                    compilation_3_res.compilation_wf_circuit
+                      |> EConstr.Vars.liftn 2 4
+                      |> econstr_substl_opt sigma [None; Some (EConstr.mkRel 1); Some (EConstr.mkRel 2)]
+                  )
+                ))
+                inputs
+                u
+                v
+                w
+                compilation_1.compilation_eval_circuit
+                (EConstr.mkLambda (EConstr.anonR,
+                  mk_circuit_type env
+                    n
+                    k,
+                  EConstr.mkLambda (EConstr.anonR,
+                    mk_circuit_wf env
+                      (n |> EConstr.Vars.lift 1)
+                      (k |> EConstr.Vars.lift 1)
+                      (EConstr.mkRel 1),
+                    EConstr.mkLambda (EConstr.anonR,
+                      mk_eq_type env
+                        (mk_vector_type env (mk_bool_type env) (k |> EConstr.Vars.lift 2))
+                        (mk_circuit_eval env
+                          (n |> EConstr.Vars.lift 2)
+                          (k |> EConstr.Vars.lift 2)
+                          (EConstr.mkRel 2)
+                          (inputs |> EConstr.Vars.lift 2))
+                        (v |> EConstr.Vars.lift 2),
+                      compilation_3_res.compilation_eval_circuit
+                        |> EConstr.Vars.liftn 3 4
+                        |> econstr_substl_opt sigma [Some (EConstr.mkRel 1); Some (EConstr.mkRel 2); Some (EConstr.mkRel 3)]
+                    )
+                  )
+                ));
+            compilation_circuit_erased =
+              mk_circuit_comp_select env
+                n
+                m
+                k
+                l
+                compilation_1.compilation_circuit_erased
+                (EConstr.mkLambda (EConstr.anonR,
+                  mk_circuit_type env
+                    n
+                    m,
+                  compilation_2_res.compilation_circuit_erased
+                    |> EConstr.Vars.liftn 1 3
+                    |> econstr_substl_opt sigma [None; Some (EConstr.mkRel 1)]
+                ))
+                (EConstr.mkLambda (EConstr.anonR,
+                  mk_circuit_type env
+                    n
+                    k,
+                  compilation_3_res.compilation_circuit_erased
+                    |> EConstr.Vars.liftn 1 4
+                    |> econstr_substl_opt sigma [None; None; Some (EConstr.mkRel 1)]
+                ));
+            compilation_eq_circuit_erased =
+              mk_circuit_comp_select_cong env
+                n
+                m
+                k
+                l
+                compilation_1.compilation_circuit_erased
+                compilation_1.compilation_circuit
+                (EConstr.mkLambda (EConstr.anonR,
+                  mk_circuit_type env
+                    n
+                    m,
+                  compilation_2_res.compilation_circuit_erased
+                    |> EConstr.Vars.liftn 1 3
+                    |> econstr_substl_opt sigma [None; Some (EConstr.mkRel 1)]
+                ))
+                (EConstr.mkLambda (EConstr.anonR,
+                  mk_circuit_type env
+                    n
+                    m,
+                  compilation_2_res.compilation_circuit
+                    |> EConstr.Vars.liftn 1 3
+                    |> econstr_substl_opt sigma [None; Some (EConstr.mkRel 1)]
+                ))
+                (EConstr.mkLambda (EConstr.anonR,
+                  mk_circuit_type env
+                    n
+                    k,
+                  compilation_3_res.compilation_circuit_erased
+                    |> EConstr.Vars.liftn 1 4
+                    |> econstr_substl_opt sigma [None; None; Some (EConstr.mkRel 1)]
+                ))
+                (EConstr.mkLambda (EConstr.anonR,
+                  mk_circuit_type env
+                    n
+                    k,
+                  compilation_3_res.compilation_circuit
+                    |> EConstr.Vars.liftn 1 4
+                    |> econstr_substl_opt sigma [None; None; Some (EConstr.mkRel 1)]
+                ))
+                compilation_1.compilation_wf_circuit
+                compilation_1.compilation_eq_circuit_erased
+                (EConstr.mkLambda (EConstr.anonR,
+                  mk_circuit_type env
+                    n
+                    m,
+                  EConstr.mkLambda (EConstr.anonR,
+                    mk_circuit_wf env
+                      (n |> EConstr.Vars.lift 1)
+                      (m |> EConstr.Vars.lift 1)
+                      (EConstr.mkRel 1),
+                    compilation_2_res.compilation_eq_circuit_erased
+                      |> EConstr.Vars.liftn 2 3
+                      |> econstr_substl_opt sigma [Some (EConstr.mkRel 1); Some (EConstr.mkRel 2)]
+                  )
+                ))
+                (EConstr.mkLambda (EConstr.anonR,
+                  mk_circuit_type env
+                    n
+                    k,
+                  EConstr.mkLambda (EConstr.anonR,
+                    mk_circuit_wf env
+                      (n |> EConstr.Vars.lift 1)
+                      (k |> EConstr.Vars.lift 1)
+                      (EConstr.mkRel 1),
+                    compilation_3_res.compilation_eq_circuit_erased
+                      |> EConstr.Vars.liftn 2 4
+                      |> econstr_substl_opt sigma [None; Some (EConstr.mkRel 1); Some (EConstr.mkRel 2)]
+                  )
+                ));
+          }
+        )
+    )
+
 let rec create_compilations (env : Environ.env) (sigma : Evd.evar_map) (context_encoders : encoder option list) (context_reprs : repr list) (context_compilations : compilation option list) (input_encoder : encoder) (c : EConstr.t) : (repr * compilation) Seq.t =
   Feedback.msg_info Pp.(str "create_compilations" ++ spc () ++ Printer.pr_econstr_env env sigma c);
   let c = Tacred.hnf_constr0 env sigma c in
@@ -1072,10 +1912,10 @@ let rec create_compilations (env : Environ.env) (sigma : Evd.evar_map) (context_
         (create_compilations
           (env |> EConstr.push_rel (Context.Rel.Declaration.LocalAssum (EConstr.anonR, c_1)))
           sigma
-          (None :: (context_encoders |> List.map (Option.map (lift_encoder 1))))
+          (None :: (context_encoders |> List.map (Option.map (encoder_lift 1))))
           (ReprRaw :: context_reprs)
-          (None :: (context_compilations |> List.map (Option.map (lift_compilation 1))))
-          (input_encoder |> lift_encoder 1)
+          (None :: (context_compilations |> List.map (Option.map (compilation_lift 1))))
+          (input_encoder |> encoder_lift 1)
           c_2
           |> Seq.map (fun (c_2_repr, c_2_compilation) ->
             (
@@ -1112,11 +1952,11 @@ let rec create_compilations (env : Environ.env) (sigma : Evd.evar_map) (context_
               None ::
               None ::
               Some {encoder_len = EConstr.mkRel 2; encoder_encode = EConstr.mkRel 1} ::
-              (context_encoders |> List.map (Option.map (lift_encoder 3)))
+              (context_encoders |> List.map (Option.map (encoder_lift 3)))
             )
             (ReprRaw :: ReprRaw :: ReprRaw :: context_reprs)
-            (None :: None :: None :: (context_compilations |> List.map (Option.map (lift_compilation 3))))
-            (input_encoder |> lift_encoder 3)
+            (None :: None :: None :: (context_compilations |> List.map (Option.map (compilation_lift 3))))
+            (input_encoder |> encoder_lift 3)
             (c_2 |> EConstr.Vars.liftn 3 2 |> EConstr.Vars.subst1 (EConstr.mkRel 3))
             |> Seq.map (fun (c_2_repr, c_2_compilation) ->
               (
@@ -1147,9 +1987,9 @@ let rec create_compilations (env : Environ.env) (sigma : Evd.evar_map) (context_
             |> Seq.flat_map (fun c_1_repr ->
               let c_1_compilation_type =
                 get_compilation_type env sigma context_encoders input_encoder c_1 c_1_repr in
-              let c_1_context = c_1_compilation_type |> compilation_type_to_context c_annot in
+              let c_1_ctx = c_1_compilation_type |> compilation_type_to_context c_annot in
               create_compilations
-                (env |> EConstr.push_rel_context c_1_context)
+                (env |> EConstr.push_rel_context c_1_ctx)
                 sigma
                 (
                   None ::
@@ -1158,7 +1998,7 @@ let rec create_compilations (env : Environ.env) (sigma : Evd.evar_map) (context_
                   None ::
                   None ::
                   None ::
-                  (context_encoders |> List.map (Option.map (lift_encoder 6)))
+                  (context_encoders |> List.map (Option.map (encoder_lift 6)))
                 )
                 (
                   ReprRaw ::
@@ -1183,22 +2023,22 @@ let rec create_compilations (env : Environ.env) (sigma : Evd.evar_map) (context_
                     compilation_circuit_erased = EConstr.mkRel 2;
                     compilation_eq_circuit_erased = EConstr.mkRel 1;
                   } ::
-                  (context_compilations |> List.map (Option.map (lift_compilation 6)))
+                  (context_compilations |> List.map (Option.map (compilation_lift 6)))
                 )
-                (input_encoder |> lift_encoder 6)
+                (input_encoder |> encoder_lift 6)
                 (c_2 |> EConstr.Vars.liftn 6 2 |> EConstr.Vars.subst1 (EConstr.mkRel 6))
                 |> Seq.map (fun (c_2_repr, c_2_compilation) ->
                   (
                     ReprFunctional (c_1_repr, c_2_repr),
                     {
                       compilation_orig =
-                        EConstr.it_mkLambda_or_LetIn c_2_compilation.compilation_orig c_1_context;
+                        EConstr.it_mkLambda_or_LetIn c_2_compilation.compilation_orig c_1_ctx;
                       compilation_circuit =
-                        EConstr.it_mkLambda_or_LetIn c_2_compilation.compilation_circuit c_1_context;
+                        EConstr.it_mkLambda_or_LetIn c_2_compilation.compilation_circuit c_1_ctx;
                       compilation_wf_circuit =
-                        EConstr.it_mkLambda_or_LetIn c_2_compilation.compilation_wf_circuit c_1_context;
+                        EConstr.it_mkLambda_or_LetIn c_2_compilation.compilation_wf_circuit c_1_ctx;
                       compilation_eval_circuit =
-                        EConstr.it_mkLambda_or_LetIn c_2_compilation.compilation_eval_circuit c_1_context;
+                        EConstr.it_mkLambda_or_LetIn c_2_compilation.compilation_eval_circuit c_1_ctx;
                       compilation_circuit_erased =
                         EConstr.mkLambda (EConstr.anonR,
                           c_1_compilation_type.compilation_circuit_erased
@@ -1220,7 +2060,7 @@ let rec create_compilations (env : Environ.env) (sigma : Evd.evar_map) (context_
                             ]
                         );
                       compilation_eq_circuit_erased =
-                        EConstr.it_mkLambda_or_LetIn c_2_compilation.compilation_eq_circuit_erased c_1_context;
+                        EConstr.it_mkLambda_or_LetIn c_2_compilation.compilation_eq_circuit_erased c_1_ctx;
                     }
                   )
                 )
@@ -1231,7 +2071,7 @@ let rec create_compilations (env : Environ.env) (sigma : Evd.evar_map) (context_
       let c_type_encoder = create_encoder env sigma context_encoders c_type in
       match c_type_encoder with
       | Some c_type_encoder ->
-        let ((ind, constructor_1_i_succ), _) = c_head |> EConstr.destConstruct sigma in
+        let ((ind, constructor_1_i_succ), u) = c_head |> EConstr.destConstruct sigma in
         let (mib, mip) = Inductive.lookup_mind_specif env ind in
         let constructor_1_i = constructor_1_i_succ - 1 in
         let params, args = CArray.chop mib.mind_nparams c_args in
@@ -1249,14 +2089,14 @@ let rec create_compilations (env : Environ.env) (sigma : Evd.evar_map) (context_
               |> List.map (create_encoder env sigma context_encoders)
               |> List.map Option.get
           ) in
-        let constructor_type_lens =
+        let constructor_types_len =
           constructor_types_hyp_encoders
             |> Array.map (fun constructor_type_hyp_encoders ->
               List.fold_right (fun len_1 len_2 ->
                 mk_nat_add env len_1.encoder_len len_2
               ) constructor_type_hyp_encoders (to_nat_constr env 0)
             ) in
-        let constructor_1_types_hyp_encoders = constructor_types_hyp_encoders.(constructor_1_i) in
+        let constructor_1_type_hyp_encoders = constructor_types_hyp_encoders.(constructor_1_i) in
         args
           |> Array.to_list
           |> List.map (fun arg ->
@@ -1267,9 +2107,16 @@ let rec create_compilations (env : Environ.env) (sigma : Evd.evar_map) (context_
           )
           |> seq_product_list
           |> Seq.map (fun arg_compilations ->
+            let c_compilation_orig =
+              EConstr.mkApp (
+                EConstr.mkConstructU ((ind, constructor_1_i_succ), u),
+                (Array.append
+                  params
+                  (arg_compilations |> CArray.map_of_list (fun arg_compilation -> arg_compilation.compilation_orig)))
+              ) in
             (
               ReprTransformed,
-              (constructor_type_lens
+              (constructor_types_len
                 |> Array.mapi (fun constructor_2_i constructor_2_type_len ->
                   if constructor_2_i = constructor_1_i then
                     List.fold_right
@@ -1283,10 +2130,10 @@ let rec create_compilations (env : Environ.env) (sigma : Evd.evar_map) (context_
                               encoder_1.encoder_len
                               encoder_2.encoder_len
                               encoder_1.encoder_encode
-                              encoder_2.encoder_encode
+                              encoder_2.encoder_encode;
                         },
                         mk_compilation_combine env
-                          c
+                          c_compilation_orig
                           input_encoder.encoder_len
                           encoder_1.encoder_len
                           encoder_2.encoder_len
@@ -1297,14 +2144,17 @@ let rec create_compilations (env : Environ.env) (sigma : Evd.evar_map) (context_
                           encoder_2.encoder_encode
                       )
                       (
-                        CList.map2_i (fun i constructor_1_types_hyp_encoder arg_compilation ->
+                        List.map2 (fun constructor_1_type_hyp_encoder arg_compilation ->
                           {
-                            encoder_len = constructor_1_types_hyp_encoder.encoder_len;
+                            encoder_len = constructor_1_type_hyp_encoder.encoder_len;
                             encoder_encode =
-                              EConstr.mkApp (constructor_1_types_hyp_encoder.encoder_encode, [|args.(i)|]);
+                              EConstr.mkApp (
+                                constructor_1_type_hyp_encoder.encoder_encode,
+                                [|arg_compilation.compilation_orig|]
+                              );
                           },
                           arg_compilation
-                        ) 0 constructor_1_types_hyp_encoders arg_compilations
+                        ) constructor_1_type_hyp_encoders arg_compilations
                       )
                       (
                         {
@@ -1312,7 +2162,7 @@ let rec create_compilations (env : Environ.env) (sigma : Evd.evar_map) (context_
                           encoder_encode = to_vector_constr env (mk_bool_type env) [];
                         },
                         mk_compilation_const env
-                          c
+                          c_compilation_orig
                           (to_nat_constr env 0)
                           input_encoder.encoder_len
                           (to_vector_constr env (mk_bool_type env) [])
@@ -1320,21 +2170,23 @@ let rec create_compilations (env : Environ.env) (sigma : Evd.evar_map) (context_
                       )
                   else
                     let placeholder =
-                      mk_vector_repeat env (mk_bool_type env) (to_bool_constr env false) constructor_2_type_len in
+                      mk_vector_repeat env
+                        (mk_bool_type env)
+                        (to_bool_constr env false)
+                        constructor_2_type_len in
                     {
                       encoder_len = constructor_2_type_len;
-                      encoder_encode =
-                        mk_vector_repeat env (mk_bool_type env) (to_bool_constr env false) constructor_2_type_len;
+                      encoder_encode = placeholder;
                     },
                     mk_compilation_const env
-                      c
+                      c_compilation_orig
                       constructor_2_type_len
                       input_encoder.encoder_len
                       placeholder
                       input_encoder.encoder_encode
                 )
                 |> Array.to_list
-                |> reduce_right_i (fun i (encoder_1, compilation_1) (encoder_2, compilation_2) ->
+                |> reduce_right_i (fun constructor_2_i (encoder_1, compilation_1) (encoder_2, compilation_2) ->
                   {
                     encoder_len =
                       mk_nat_add env (to_nat_constr env 1) (mk_nat_add env encoder_1.encoder_len encoder_2.encoder_len);
@@ -1343,7 +2195,7 @@ let rec create_compilations (env : Environ.env) (sigma : Evd.evar_map) (context_
                         (mk_bool_type env)
                         (to_nat_constr env 1)
                         (mk_nat_add env encoder_1.encoder_len encoder_2.encoder_len)
-                        (to_vector_constr env (mk_bool_type env) [to_bool_constr env (i = constructor_1_i)])
+                        (to_vector_constr env (mk_bool_type env) [to_bool_constr env (constructor_2_i = constructor_1_i)])
                         (mk_vector_app env
                           (mk_bool_type env)
                           encoder_1.encoder_len
@@ -1352,18 +2204,18 @@ let rec create_compilations (env : Environ.env) (sigma : Evd.evar_map) (context_
                           encoder_2.encoder_encode)
                   },
                   mk_compilation_combine env
-                    c
+                    c_compilation_orig
                     input_encoder.encoder_len
                     (to_nat_constr env 1)
                     (mk_nat_add env encoder_1.encoder_len encoder_2.encoder_len)
                     (mk_compilation_const env
-                      c
+                      c_compilation_orig
                       (to_nat_constr env 1)
                       input_encoder.encoder_len
-                      (to_vector_constr env (mk_bool_type env) [to_bool_constr env (i = constructor_1_i)])
+                      (to_vector_constr env (mk_bool_type env) [to_bool_constr env (constructor_2_i = constructor_1_i)])
                       input_encoder.encoder_encode)
                     (mk_compilation_combine env
-                      c
+                      c_compilation_orig
                       input_encoder.encoder_len
                       encoder_1.encoder_len
                       encoder_2.encoder_len
@@ -1373,7 +2225,7 @@ let rec create_compilations (env : Environ.env) (sigma : Evd.evar_map) (context_
                       encoder_1.encoder_encode
                       encoder_2.encoder_encode)
                     input_encoder.encoder_encode
-                    (to_vector_constr env (mk_bool_type env) [to_bool_constr env (i = constructor_1_i)])
+                    (to_vector_constr env (mk_bool_type env) [to_bool_constr env (constructor_2_i = constructor_1_i)])
                     (mk_vector_app env
                       (mk_bool_type env)
                       encoder_1.encoder_len
@@ -1602,244 +2454,697 @@ let rec create_compilations (env : Environ.env) (sigma : Evd.evar_map) (context_
               (Array.init (List.length arity_ctx) (fun i -> EConstr.mkRel (List.length arity_ctx - i)))
           ) in
         create_compilations env sigma context_encoders context_reprs context_compilations input_encoder c_scrutinee
-          |> Seq.filter_map (fun (c_scrutinee_repr, c_scrutinee_compilation) ->
-            if c_scrutinee_repr = ReprRaw then Some c_scrutinee_compilation else None
-          )
-          |> Seq.flat_map (fun c_scrutinee_compilation ->
-            enumerate_reprs
-              (env |> EConstr.push_rel_context (Context.Rel.Declaration.LocalAssum (EConstr.anonR, scrutinee_type_arity_ctx) :: arity_ctx))
-              sigma
-              (None :: (arity_ctx |> List.map (fun _ -> None)) @ (context_encoders |> List.map (Option.map (lift_encoder (1 + List.length arity_ctx)))))
-              c_return_t
-              |> List.to_seq
-              |> Seq.flat_map (fun c_return_t_repr ->
-                let c_return_t_compilation_type =
-                  get_compilation_type
-                    (env |> EConstr.push_rel_context (Context.Rel.Declaration.LocalAssum (EConstr.anonR, scrutinee_type_arity_ctx) :: arity_ctx))
-                    sigma
-                    (None :: (arity_ctx |> List.map (fun _ -> None)) @ (context_encoders |> List.map (Option.map (lift_encoder (1 + List.length arity_ctx)))))
-                    (input_encoder |> lift_encoder (1 + List.length arity_ctx))
-                    c_return_t
-                    c_return_t_repr in
-                Array.map2 (fun (c_br_annots, c_br_t) (constructor_type_ctx, _) ->
-                  create_compilations
-                    (env |> EConstr.push_rel_context constructor_type_ctx)
-                    sigma
-                    ((constructor_type_ctx |> List.map (fun _ -> None)) @ (context_encoders |> List.map (Option.map (lift_encoder (List.length constructor_type_ctx)))))
-                    ((constructor_type_ctx |> List.map (fun _ -> ReprRaw)) @ context_reprs)
-                    ((constructor_type_ctx |> List.map (fun _ -> None)) @ (context_compilations |> List.map (Option.map (lift_compilation (List.length constructor_type_ctx)))))
-                    (input_encoder |> lift_encoder (List.length constructor_type_ctx))
-                    c_br_t
-                  |> Seq.filter_map (fun (c_br_t_repr, c_br_t_compilation) ->
-                    if c_br_t_repr = c_return_t_repr then Some (c_br_annots, c_br_t_compilation) else None
-                  )
-                ) c_brs constructor_types_ctx_concl
-                  |> seq_product_array
-                  |> Seq.flat_map (fun c_brs_annots_t_compilation ->
-                    let c_compilation_gen_orig =
-                      EConstr.mkCase (
-                        ci,
-                        u,
-                        c_params |> Array.map (EConstr.Vars.lift (1 + List.length arity_ctx)),
-                        (
-                          (
-                            c_return_annots,
-                            c_return_t_compilation_type.compilation_orig
-                              |> EConstr.Vars.liftn (1 + List.length arity_ctx) (0 + 1 + List.length arity_ctx + 1)
-                              |> EConstr.Vars.substl []
-                          ),
-                          EConstr.ERelevance.relevant
-                        ),
-                        Constr.NoInvert,
-                        EConstr.mkRel 1,
-                        c_brs_annots_t_compilation |> Array.map (fun (c_br_annots, c_br_t_compilation) ->
-                          (
-                            c_br_annots,
-                            c_br_t_compilation.compilation_orig
-                              |> EConstr.Vars.liftn (1 + List.length arity_ctx) (Array.length c_br_annots + 1)
-                          )
-                        )
-                      ) in
-                    let c_compilation_gen_circuit =
-                      EConstr.mkCase (
-                        ci,
-                        u,
-                        c_params |> Array.map (EConstr.Vars.lift (1 + List.length arity_ctx)),
-                        (
-                          (
-                            c_return_annots,
-                            c_return_t_compilation_type.compilation_circuit
-                              |> EConstr.Vars.liftn (1 + List.length arity_ctx) (1 + 1 + List.length arity_ctx + 1)
-                              |> EConstr.Vars.substl [
-                                c_compilation_gen_orig
-                                  |> EConstr.Vars.liftn (1 + List.length arity_ctx) (1 + List.length arity_ctx + 1);
-                              ]
-                          ),
-                          EConstr.ERelevance.relevant
-                        ),
-                        Constr.NoInvert,
-                        EConstr.mkRel 1,
-                        c_brs_annots_t_compilation |> Array.map (fun (c_br_annots, c_br_t_compilation) ->
-                          (
-                            c_br_annots,
-                            c_br_t_compilation.compilation_circuit
-                              |> EConstr.Vars.liftn (1 + List.length arity_ctx) (Array.length c_br_annots + 1)
-                          )
-                        )
-                      ) in
-                    let c_compilation_gen_wf_circuit =
-                      EConstr.mkCase (
-                        ci,
-                        u,
-                        c_params |> Array.map (EConstr.Vars.lift (1 + List.length arity_ctx)),
-                        (
-                          (
-                            c_return_annots,
-                            c_return_t_compilation_type.compilation_wf_circuit
-                              |> EConstr.Vars.liftn (1 + List.length arity_ctx) (2 + 1 + List.length arity_ctx + 1)
-                              |> EConstr.Vars.substl [
-                                c_compilation_gen_circuit
-                                  |> EConstr.Vars.liftn (1 + List.length arity_ctx) (1 + List.length arity_ctx + 1);
-                                c_compilation_gen_orig
-                                  |> EConstr.Vars.liftn (1 + List.length arity_ctx) (1 + List.length arity_ctx + 1);
-                              ]
-                          ),
-                          EConstr.ERelevance.relevant
-                        ),
-                        Constr.NoInvert,
-                        EConstr.mkRel 1,
-                        c_brs_annots_t_compilation |> Array.map (fun (c_br_annots, c_br_t_compilation) ->
-                          (
-                            c_br_annots,
-                            c_br_t_compilation.compilation_wf_circuit
-                              |> EConstr.Vars.liftn (1 + List.length arity_ctx) (Array.length c_br_annots + 1)
-                          )
-                        )
-                      ) in
-                    let c_compilation_gen_eval_circuit =
-                      EConstr.mkCase (
-                        ci,
-                        u,
-                        c_params |> Array.map (EConstr.Vars.lift (1 + List.length arity_ctx)),
-                        (
-                          (
-                            c_return_annots,
-                            c_return_t_compilation_type.compilation_eval_circuit
-                              |> EConstr.Vars.liftn (1 + List.length arity_ctx) (3 + 1 + List.length arity_ctx + 1)
-                              |> EConstr.Vars.substl [
-                                c_compilation_gen_wf_circuit
-                                  |> EConstr.Vars.liftn (1 + List.length arity_ctx) (1 + List.length arity_ctx + 1);
-                                c_compilation_gen_circuit
-                                  |> EConstr.Vars.liftn (1 + List.length arity_ctx) (1 + List.length arity_ctx + 1);
-                                c_compilation_gen_orig
-                                  |> EConstr.Vars.liftn (1 + List.length arity_ctx) (1 + List.length arity_ctx + 1);
-                              ]
-                          ),
-                          EConstr.ERelevance.relevant
-                        ),
-                        Constr.NoInvert,
-                        EConstr.mkRel 1,
-                        c_brs_annots_t_compilation |> Array.map (fun (c_br_annots, c_br_t_compilation) ->
-                          (
-                            c_br_annots,
-                            c_br_t_compilation.compilation_eval_circuit
-                              |> EConstr.Vars.liftn (1 + List.length arity_ctx) (Array.length c_br_annots + 1)
-                          )
-                        )
-                      ) in
-                    let c_compilation_gen_circuit_erased =
-                      EConstr.mkCase (
-                        ci,
-                        u,
-                        c_params |> Array.map (EConstr.Vars.lift (1 + List.length arity_ctx)),
-                        (
-                          (
-                            c_return_annots,
-                            c_return_t_compilation_type.compilation_circuit_erased
-                              |> EConstr.Vars.liftn (1 + List.length arity_ctx) (4 + 1 + List.length arity_ctx + 1)
-                              |> EConstr.Vars.substl [
-                                c_compilation_gen_eval_circuit
-                                  |> EConstr.Vars.liftn (1 + List.length arity_ctx) (1 + List.length arity_ctx + 1);
-                                c_compilation_gen_wf_circuit
-                                  |> EConstr.Vars.liftn (1 + List.length arity_ctx) (1 + List.length arity_ctx + 1);
-                                c_compilation_gen_circuit
-                                  |> EConstr.Vars.liftn (1 + List.length arity_ctx) (1 + List.length arity_ctx + 1);
-                                c_compilation_gen_orig
-                                  |> EConstr.Vars.liftn (1 + List.length arity_ctx) (1 + List.length arity_ctx + 1);
-                              ]
-                          ),
-                          EConstr.ERelevance.relevant
-                        ),
-                        Constr.NoInvert,
-                        EConstr.mkRel 1,
-                        c_brs_annots_t_compilation |> Array.map (fun (c_br_annots, c_br_t_compilation) ->
-                          (
-                            c_br_annots,
-                            c_br_t_compilation.compilation_circuit_erased
-                              |> EConstr.Vars.liftn (1 + List.length arity_ctx) (Array.length c_br_annots + 1)
-                          )
-                        )
-                      ) in
-                    let c_compilation_gen_eq_circuit_erased =
-                      EConstr.mkCase (
-                        ci,
-                        u,
-                        c_params |> Array.map (EConstr.Vars.lift (1 + List.length arity_ctx)),
-                        (
-                          (
-                            c_return_annots,
-                            c_return_t_compilation_type.compilation_eq_circuit_erased
-                              |> EConstr.Vars.liftn (1 + List.length arity_ctx) (5 + 1 + List.length arity_ctx + 1)
-                              |> EConstr.Vars.substl [
-                                c_compilation_gen_circuit_erased
-                                  |> EConstr.Vars.liftn (1 + List.length arity_ctx) (1 + List.length arity_ctx + 1);
-                                c_compilation_gen_eval_circuit
-                                  |> EConstr.Vars.liftn (1 + List.length arity_ctx) (1 + List.length arity_ctx + 1);
-                                c_compilation_gen_wf_circuit
-                                  |> EConstr.Vars.liftn (1 + List.length arity_ctx) (1 + List.length arity_ctx + 1);
-                                c_compilation_gen_circuit
-                                  |> EConstr.Vars.liftn (1 + List.length arity_ctx) (1 + List.length arity_ctx + 1);
-                                c_compilation_gen_orig
-                                  |> EConstr.Vars.liftn (1 + List.length arity_ctx) (1 + List.length arity_ctx + 1);
-                              ]
-                          ),
-                          EConstr.ERelevance.relevant
-                        ),
-                        Constr.NoInvert,
-                        EConstr.mkRel 1,
-                        c_brs_annots_t_compilation |> Array.map (fun (c_br_annots, c_br_t_compilation) ->
-                          (
-                            c_br_annots,
-                            c_br_t_compilation.compilation_eq_circuit_erased
-                              |> EConstr.Vars.liftn (1 + List.length arity_ctx) (Array.length c_br_annots + 1)
-                          )
-                        )
-                      ) in
-                    Seq.return (
-                      c_return_t_repr,
-                      {
-                        compilation_orig =
-                          c_compilation_gen_orig
-                            |> econstr_substl_opt sigma (Some c_scrutinee_compilation.compilation_orig :: (arity_ctx |> List.map (fun _ -> None)));
-                        compilation_circuit =
-                          c_compilation_gen_circuit
-                            |> econstr_substl_opt sigma (Some c_scrutinee_compilation.compilation_orig :: (arity_ctx |> List.map (fun _ -> None)));
-                        compilation_wf_circuit =
-                          c_compilation_gen_wf_circuit
-                            |> econstr_substl_opt sigma (Some c_scrutinee_compilation.compilation_orig :: (arity_ctx |> List.map (fun _ -> None)));
-                        compilation_eval_circuit =
-                          c_compilation_gen_eval_circuit
-                            |> econstr_substl_opt sigma (Some c_scrutinee_compilation.compilation_orig :: (arity_ctx |> List.map (fun _ -> None)));
-                        compilation_circuit_erased =
-                          c_compilation_gen_circuit_erased
-                            |> econstr_substl_opt sigma (Some c_scrutinee_compilation.compilation_orig :: (arity_ctx |> List.map (fun _ -> None)));
-                        compilation_eq_circuit_erased =
-                          c_compilation_gen_eq_circuit_erased
-                            |> econstr_substl_opt sigma (Some c_scrutinee_compilation.compilation_orig :: (arity_ctx |> List.map (fun _ -> None)));
-                      }
+          |> Seq.flat_map (fun (c_scrutinee_repr, c_scrutinee_compilation) ->
+            if c_scrutinee_repr = ReprTransformed && c_return_t |> EConstr.Vars.noccurn sigma 1 then
+              let c_scrutinee_encoder =
+                create_encoder env sigma context_encoders scrutinee_type_arity_ctx |> Option.get in
+              let c_scrutinee_compilation_type =
+                get_compilation_type env sigma context_encoders input_encoder scrutinee_type_arity_ctx ReprTransformed in
+              let c_scrutinee_ctx = c_scrutinee_compilation_type |> compilation_type_to_context EConstr.anonR in
+              let c_return_t_unlifted = c_return_t |> econstr_substl_opt sigma [None] in
+              let c_return_t_unlifted_encoder = create_encoder env sigma context_encoders c_return_t_unlifted in
+              match c_return_t_unlifted_encoder with
+              | Some c_return_t_unlifted_encoder ->
+                let c_return_t_unlifted_compilation_type =
+                  get_compilation_type env sigma context_encoders input_encoder c_return_t_unlifted ReprTransformed in
+                let constructor_types_hyps_concl =
+                  mip.mind_nf_lc |> Array.map (fun (ctx, concl) ->
+                    decompose_arrows sigma (
+                      EConstr.Vars.substl
+                        (List.rev (Array.to_list c_params))
+                        (EConstr.of_constr (Term.it_mkProd_or_LetIn concl (ctx |> List.take (List.length ctx - mib.mind_nparams))))
                     )
+                  ) in
+                let constructor_types_hyp_encoders =
+                  constructor_types_hyps_concl |> Array.map (fun (constructor_type_hyps, _) ->
+                    constructor_type_hyps
+                      |> List.map (create_encoder env sigma context_encoders)
+                      |> List.map Option.get
+                  ) in
+                (* let constructor_types_len =
+                  constructor_types_hyp_encoders
+                    |> Array.map (fun constructor_type_hyp_encoders ->
+                      List.fold_right (fun len_1 len_2 ->
+                        mk_nat_add env len_1.encoder_len len_2
+                      ) constructor_type_hyp_encoders (to_nat_constr env 0)
+                    ) in *)
+                CArray.map2_i (fun constructor_1_i (constructor_1_type_ctx, _) (_, c_br_1_t) ->
+                  (CArray.map3_i (fun constructor_2_i (constructor_2_type_ctx, _) constructor_2_type_hyp_encoders (_, c_br_2_t) ->
+                    let arg_encoders =
+                      constructor_2_type_hyp_encoders |> List.mapi (fun arg_i constructor_2_type_hyp_encoder ->
+                        {
+                          encoder_len =
+                            constructor_2_type_hyp_encoder.encoder_len
+                              |> EConstr.Vars.lift (List.length constructor_1_type_ctx);
+                          encoder_encode =
+                            EConstr.mkApp (
+                              constructor_2_type_hyp_encoder.encoder_encode
+                                |> EConstr.Vars.lift (List.length constructor_1_type_ctx),
+                              [|EConstr.mkRel (List.length constructor_1_type_ctx - arg_i)|]
+                            );
+                        }
+                      ) in
+                    let constructor_2_encoder, g =
+                      CList.fold_right_i
+                        (fun arg_i arg_encoder (args_encoder, g) ->
+                          {
+                            encoder_len =
+                              mk_nat_add env arg_encoder.encoder_len args_encoder.encoder_len;
+                            encoder_encode =
+                              mk_vector_app env
+                                (mk_bool_type env)
+                                arg_encoder.encoder_len
+                                args_encoder.encoder_len
+                                arg_encoder.encoder_encode
+                                args_encoder.encoder_encode;
+                          },
+                          fun constructor_2_ctx constructor_2_compilation ->
+                            let arg_compilation_transforms, rest_args_compilation_transform = g constructor_2_ctx constructor_2_compilation in
+                            (* let () = Feedback.msg_info Pp.(str "arg_i" ++ spc () ++ int arg_i) in
+                            let () = Feedback.msg_info Pp.(str "arg_compilation_transforms" ++ spc () ++ int (List.length arg_compilation_transforms)) in *)
+                            let f compilation_transform =
+                              fun args_compilation ->
+                                compilation_transform (
+                                  mk_compilation_comp_suffix env
+                                    (mk_unit_tt env)
+                                    (input_encoder.encoder_len
+                                      |> EConstr.Vars.lift (List.length constructor_2_ctx + List.length constructor_1_type_ctx))
+                                    (arg_encoder.encoder_len
+                                      |> EConstr.Vars.lift (List.length constructor_2_ctx))
+                                    (args_encoder.encoder_len
+                                      |> EConstr.Vars.lift (List.length constructor_2_ctx))
+                                    args_compilation
+                                    (input_encoder.encoder_encode
+                                      |> EConstr.Vars.lift (List.length constructor_2_ctx + List.length constructor_1_type_ctx))
+                                    (arg_encoder.encoder_encode
+                                      |> EConstr.Vars.lift (List.length constructor_2_ctx))
+                                    (args_encoder.encoder_encode
+                                      |> EConstr.Vars.lift (List.length constructor_2_ctx))
+                                ) in
+                            (fun args_compilation ->
+                              mk_compilation_comp_prefix env
+                                (EConstr.mkRel (arg_i + 1)
+                                  |> EConstr.Vars.lift (List.length constructor_2_ctx))
+                                (input_encoder.encoder_len
+                                  |> EConstr.Vars.lift (List.length constructor_2_ctx + List.length constructor_1_type_ctx))
+                                (arg_encoder.encoder_len
+                                  |> EConstr.Vars.lift (List.length constructor_2_ctx))
+                                (args_encoder.encoder_len
+                                  |> EConstr.Vars.lift (List.length constructor_2_ctx))
+                                args_compilation
+                                (input_encoder.encoder_encode
+                                  |> EConstr.Vars.lift (List.length constructor_2_ctx + List.length constructor_1_type_ctx))
+                                (arg_encoder.encoder_encode
+                                  |> EConstr.Vars.lift (List.length constructor_2_ctx))
+                                (args_encoder.encoder_encode
+                                  |> EConstr.Vars.lift (List.length constructor_2_ctx))
+                            ) ::
+                            (arg_compilation_transforms |> List.map f),
+                            f rest_args_compilation_transform
+                        )
+                        0
+                        arg_encoders
+                        (
+                          {
+                            encoder_len = to_nat_constr env 0;
+                            encoder_encode = to_vector_constr env (mk_bool_type env) [];
+                          },
+                          fun _ _ ->
+                            [],
+                            (fun args_compilation -> args_compilation)
+                        ) in
+                    (if constructor_2_i = constructor_1_i then
+                      constructor_2_encoder
+                    else
+                      let placeholder =
+                        mk_vector_repeat env
+                          (mk_bool_type env)
+                          (to_bool_constr env false)
+                          constructor_2_encoder.encoder_len in
+                      {
+                        encoder_len = constructor_2_encoder.encoder_len;
+                        encoder_encode = placeholder;
+                      }),
+                    fun constructor_2_ctx constructor_2_compilation ->
+                      let arg_compilation_transforms, _ = g constructor_2_ctx constructor_2_compilation in
+                      let arg_compilations =
+                        arg_compilation_transforms |> List.map (fun arg_compilation_transform ->
+                          arg_compilation_transform constructor_2_compilation
+                        ) in
+                      Feedback.msg_info Pp.(str "constructor_2_ctx" ++ spc () ++ int (List.length constructor_2_ctx));
+                      Feedback.msg_info Pp.(str "constructor_2_type_ctx" ++ spc () ++ int (List.length constructor_2_type_ctx));
+                      Feedback.msg_info Pp.(str "c_br_2_t" ++ spc () ++ Printer.pr_econstr_env env sigma c_br_2_t);
+                      (* Feedback.msg_info Pp.(str "ARG" ++ spc () ++ Printer.pr_econstr_env env sigma (List.nth arg_compilations 0).compilation_orig);
+                      Feedback.msg_info Pp.(str "ARG" ++ spc () ++ Printer.pr_econstr_env env sigma (List.nth arg_compilations 1).compilation_orig);
+                      Feedback.msg_info Pp.(str "ARG" ++ spc () ++ Printer.pr_econstr_env env sigma (List.nth arg_compilations 0).compilation_circuit);
+                      Feedback.msg_info Pp.(str "ARG" ++ spc () ++ Printer.pr_econstr_env env sigma (List.nth arg_compilations 1).compilation_circuit); *)
+                      create_compilations
+                        (env |> EConstr.push_rel_context (constructor_2_type_ctx @ constructor_2_ctx @ constructor_1_type_ctx))
+                        sigma
+                        (
+                          (constructor_2_type_ctx |> List.map (fun _ -> None)) @
+                          (constructor_2_ctx |> List.map (fun _ -> None)) @
+                          (constructor_1_type_ctx |> List.map (fun _ -> None)) @
+                          (context_encoders |> List.map (Option.map (encoder_lift (List.length constructor_2_type_ctx + List.length constructor_2_ctx + List.length constructor_1_type_ctx))))
+                        )
+                        (
+                          (constructor_2_type_ctx |> List.map (fun _ -> ReprTransformed)) @
+                          (constructor_2_ctx |> List.map (fun _ -> ReprRaw)) @
+                          (constructor_1_type_ctx |> List.map (fun _ -> ReprRaw)) @
+                          context_reprs
+                        )
+                        (
+                          (arg_compilations |> List.rev |> List.map (fun arg_compilation -> Some (arg_compilation |> compilation_lift (List.length constructor_2_type_ctx)))) @
+                          (constructor_2_ctx |> List.map (fun _ -> None)) @
+                          (constructor_1_type_ctx |> List.map (fun _ -> None)) @
+                          (context_compilations |> List.map (Option.map (compilation_lift (List.length constructor_2_type_ctx + List.length constructor_2_ctx + List.length constructor_1_type_ctx))))
+                        )
+                        (input_encoder
+                          |> encoder_lift (List.length constructor_2_type_ctx + List.length constructor_2_ctx + List.length constructor_1_type_ctx))
+                        (c_br_2_t
+                          |> EConstr.Vars.liftn (List.length constructor_2_ctx + List.length constructor_1_type_ctx) (List.length constructor_2_type_ctx + 1))
+                        |> Seq.filter_map (fun (c_br_t_repr, c_br_t_compilation) ->
+                          if c_br_t_repr = ReprTransformed then
+                            let () = Feedback.msg_info Pp.(str "RES" ++ spc () ++ Printer.pr_econstr_env env sigma c_br_t_compilation.compilation_orig) in
+                            Some (c_br_t_compilation |> compilation_substl_opt sigma (constructor_2_type_ctx |> List.map (fun _ -> None)))
+                          else
+                            None
+                        )
+                  ) constructor_types_ctx_concl constructor_types_hyp_encoders c_brs
+                    |> Array.to_list
+                    |> reduce_right_i (fun constructor_2_i (encoder_1, compilations_1) (encoder_2, compilations_2) ->
+                      {
+                        encoder_len =
+                          mk_nat_add env (to_nat_constr env 1) (mk_nat_add env encoder_1.encoder_len encoder_2.encoder_len);
+                        encoder_encode =
+                          mk_vector_app env
+                            (mk_bool_type env)
+                            (to_nat_constr env 1)
+                            (mk_nat_add env encoder_1.encoder_len encoder_2.encoder_len)
+                            (to_vector_constr env (mk_bool_type env) [to_bool_constr env (constructor_2_i = constructor_1_i)])
+                            (mk_vector_app env
+                              (mk_bool_type env)
+                              encoder_1.encoder_len
+                              encoder_2.encoder_len
+                              encoder_1.encoder_encode
+                              encoder_2.encoder_encode)
+                      },
+                      fun ctx compilation ->
+                        (if constructor_2_i = constructor_1_i
+                        then mk_compilation_comp_select_1
+                        else mk_compilation_comp_select_2)
+                          env
+                          sigma
+                          (input_encoder.encoder_len
+                            |> EConstr.Vars.lift (List.length ctx + List.length constructor_1_type_ctx))
+                          (encoder_1.encoder_len
+                            |> EConstr.Vars.lift (List.length ctx))
+                          (encoder_2.encoder_len
+                            |> EConstr.Vars.lift (List.length ctx))
+                          (c_return_t_unlifted_encoder.encoder_len
+                            |> EConstr.Vars.lift (List.length ctx + List.length constructor_1_type_ctx))
+                          compilation
+                          (fun ctx' compilation' -> compilations_1 (ctx' @ ctx) compilation')
+                          (fun ctx' compilation' -> compilations_2 (ctx' @ ctx) compilation')
+                          (input_encoder.encoder_encode
+                            |> EConstr.Vars.lift (List.length ctx + List.length constructor_1_type_ctx))
+                          (encoder_1.encoder_encode
+                            |> EConstr.Vars.lift (List.length ctx))
+                          (encoder_2.encoder_encode
+                            |> EConstr.Vars.lift (List.length ctx))
+                          (EConstr.mkApp (
+                            c_return_t_unlifted_encoder.encoder_encode
+                              |> EConstr.Vars.lift (List.length ctx + List.length constructor_1_type_ctx),
+                            [|c_br_1_t
+                              |> EConstr.Vars.lift (List.length ctx)|]
+                          ))
+                    )
+                    |> snd)
+                    c_scrutinee_ctx
+                    {
+                      compilation_orig = EConstr.mkRel 6;
+                      compilation_circuit = EConstr.mkRel 5;
+                      compilation_wf_circuit = EConstr.mkRel 4;
+                      compilation_eval_circuit = EConstr.mkRel 3;
+                      compilation_circuit_erased = EConstr.mkRel 2;
+                      compilation_eq_circuit_erased = EConstr.mkRel 1;
+                    }
+                    |> Seq.map (compilation_liftn (List.length constructor_1_type_ctx + List.length c_scrutinee_ctx) (List.length c_scrutinee_ctx + List.length constructor_1_type_ctx + 1))
+                    |> Seq.map (compilation_substl (
+                      (c_scrutinee_ctx |> List.mapi (fun i _ -> EConstr.mkRel (List.length constructor_1_type_ctx + i + 1))) @
+                      (constructor_1_type_ctx |> List.mapi (fun i _ -> EConstr.mkRel (i + 1)))
+                    ))
+                ) constructor_types_ctx_concl c_brs
+                |> seq_zip_strict_array
+                |> Seq.flat_map (fun c_brs_t_compilation ->
+                  let c_compilation_gen_orig =
+                    EConstr.mkCase (
+                      ci,
+                      u,
+                      c_params |> Array.map (EConstr.Vars.lift (List.length c_scrutinee_ctx)),
+                      (
+                        (
+                          c_return_annots,
+                          c_return_t_unlifted_compilation_type.compilation_orig
+                            |> EConstr.Vars.liftn (List.length c_scrutinee_ctx) (0 + 1)
+                            |> EConstr.Vars.substl []
+                            |> EConstr.Vars.lift 1
+                        ),
+                        EConstr.ERelevance.relevant
+                      ),
+                      Constr.NoInvert,
+                      EConstr.mkRel 6,
+                      Array.map2 (fun (c_br_annots, _) c_br_t_compilation ->
+                        (
+                          c_br_annots,
+                          c_br_t_compilation.compilation_orig
+                        )
+                      ) c_brs c_brs_t_compilation
+                    ) in
+                  (* Feedback.msg_info Pp.(str "A_0" ++ spc () ++ int (c_brs_t_compilation.(0).compilation_orig |> EConstr.destRel sigma)); *)
+                  Feedback.msg_info Pp.(str "HEY_1" ++ spc () ++ Printer.pr_econstr_env env sigma c_compilation_gen_orig);
+                  let c_compilation_gen_circuit_all =
+                    Array.map2 (fun (constructor_type_hyps, _) br_t_compilation ->
+                      br_t_compilation.compilation_circuit
+                        |> econstr_substl_opt sigma (constructor_type_hyps |> List.map (fun _ -> None))
+                    ) constructor_types_hyps_concl c_brs_t_compilation in
+                  let c_compilation_gen_circuit = c_compilation_gen_circuit_all.(0) in
+                  (* Feedback.msg_info Pp.(str "A_1" ++ spc () ++ Printer.pr_econstr_env env sigma (c_compilation_gen_circuit_all.(0)));
+                  Feedback.msg_info Pp.(str "A_2" ++ spc () ++ Printer.pr_econstr_env env sigma (c_compilation_gen_circuit_all.(1))); *)
+                  (* assert (c_compilation_gen_circuit_all |> Array.for_all (EConstr.eq_constr sigma c_compilation_gen_circuit)); *)
+                  Feedback.msg_info Pp.(str "HEY_2" ++ spc () ++ Printer.pr_econstr_env env sigma c_compilation_gen_circuit);
+                  let c_compilation_gen_wf_circuit_all =
+                    Array.map2 (fun (constructor_type_hyps, _) br_t_compilation ->
+                      br_t_compilation.compilation_wf_circuit
+                        |> econstr_substl_opt sigma (constructor_type_hyps |> List.map (fun _ -> None))
+                    ) constructor_types_hyps_concl c_brs_t_compilation in
+                  let c_compilation_gen_wf_circuit = c_compilation_gen_wf_circuit_all.(0) in
+                  (* assert (c_compilation_gen_wf_circuit_all |> Array.for_all (EConstr.eq_constr sigma c_compilation_gen_wf_circuit)); *)
+                  Feedback.msg_info Pp.(str "HEY_3" ++ spc () ++ Printer.pr_econstr_env env sigma c_compilation_gen_wf_circuit);
+                  let c_compilation_gen_eval_circuit =
+                    EConstr.mkApp (
+                      EConstr.mkCase (
+                        ci,
+                        u,
+                        c_params |> Array.map (EConstr.Vars.lift (List.length c_scrutinee_ctx)),
+                        (
+                          (
+                            c_return_annots,
+                            EConstr.mkProd (EConstr.anonR,
+                              mk_eq_type env
+                                (mk_vector_type env
+                                  (mk_bool_type env)
+                                  (c_scrutinee_encoder.encoder_len |> EConstr.Vars.lift (1 + List.length c_scrutinee_ctx)))
+                                (EConstr.mkApp (
+                                  c_scrutinee_encoder.encoder_encode |> EConstr.Vars.lift (1 + List.length c_scrutinee_ctx),
+                                  [|EConstr.mkRel 7|]
+                                ))
+                                (EConstr.mkApp (
+                                  c_scrutinee_encoder.encoder_encode |> EConstr.Vars.lift (1 + List.length c_scrutinee_ctx),
+                                  [|EConstr.mkRel 1|]
+                                )),
+                                c_return_t_unlifted_compilation_type.compilation_eval_circuit
+                                  |> EConstr.Vars.liftn (2 + List.length c_scrutinee_ctx) (3 + 1)
+                                  |> EConstr.Vars.substl [
+                                    c_compilation_gen_wf_circuit
+                                      |> EConstr.Vars.lift 2;
+                                    c_compilation_gen_circuit
+                                      |> EConstr.Vars.lift 2;
+                                    c_compilation_gen_orig
+                                      |> EConstr.Vars.liftn (2 + List.length c_scrutinee_ctx) (List.length c_scrutinee_ctx + 1)
+                                      |> EConstr.Vars.substl [
+                                        EConstr.mkRel 3;
+                                        EConstr.mkRel 4;
+                                        EConstr.mkRel 5;
+                                        EConstr.mkRel 6;
+                                        EConstr.mkRel 7;
+                                        EConstr.mkRel 2;
+                                      ];
+                                  ]
+                            )
+                          ),
+                          EConstr.ERelevance.relevant
+                        ),
+                        Constr.NoInvert,
+                        EConstr.mkRel 6,
+                        CArray.map3_i (fun constructor_i (constructor_type_hyps, _) (c_br_annots, _) c_br_t_compilation ->
+                          (
+                            c_br_annots,
+                            let constructor_app =
+                              EConstr.mkApp (
+                                EConstr.mkConstructU ((ind, constructor_i + 1), u),
+                                (Array.append
+                                  (c_params |> Array.map (EConstr.Vars.lift (List.length constructor_type_hyps + List.length c_scrutinee_ctx)))
+                                  (constructor_type_hyps |> List.mapi (fun i _ -> EConstr.mkRel (List.length constructor_type_hyps - i)) |> Array.of_list))
+                              ) in
+                            EConstr.mkLambda (EConstr.anonR,
+                              mk_eq_type env
+                                (mk_vector_type env
+                                  (mk_bool_type env)
+                                  (c_scrutinee_encoder.encoder_len |> EConstr.Vars.lift (List.length constructor_type_hyps + List.length c_scrutinee_ctx)))
+                                (EConstr.mkApp (
+                                  c_scrutinee_encoder.encoder_encode |> EConstr.Vars.lift (List.length constructor_type_hyps + List.length c_scrutinee_ctx),
+                                  [|EConstr.mkRel (List.length constructor_type_hyps + 6)|]
+                                ))
+                                (EConstr.mkApp (
+                                  c_scrutinee_encoder.encoder_encode |> EConstr.Vars.lift (List.length constructor_type_hyps + List.length c_scrutinee_ctx),
+                                  [|constructor_app|]
+                                )),
+                              c_br_t_compilation.compilation_eval_circuit
+                                |> EConstr.Vars.liftn (List.length constructor_type_hyps + 7) (List.length constructor_type_hyps + 8)
+                                |> EConstr.Vars.substl (
+                                  (constructor_type_hyps |> List.mapi (fun i _ -> EConstr.mkRel (1 + i + 1))) @
+                                  [
+                                    EConstr.mkRel (1 + List.length constructor_type_hyps + 1);
+                                    EConstr.mkRel (1 + List.length constructor_type_hyps + 2);
+                                    mk_eq_trans env
+                                      (mk_vector_type env
+                                        (mk_bool_type env)
+                                        (c_scrutinee_encoder.encoder_len |> EConstr.Vars.lift (1 + List.length constructor_type_hyps + List.length c_scrutinee_ctx)))
+                                      (
+                                        mk_circuit_eval env
+                                          (input_encoder.encoder_len |> EConstr.Vars.lift (1 + List.length constructor_type_hyps + List.length c_scrutinee_ctx))
+                                          (c_scrutinee_encoder.encoder_len |> EConstr.Vars.lift (1 + List.length constructor_type_hyps + List.length c_scrutinee_ctx))
+                                          (EConstr.mkRel (1 + List.length constructor_type_hyps + 5))
+                                          (input_encoder.encoder_encode |> EConstr.Vars.lift (1 + List.length constructor_type_hyps + List.length c_scrutinee_ctx))
+                                      )
+                                      (EConstr.mkApp (
+                                        c_scrutinee_encoder.encoder_encode |> EConstr.Vars.lift (1 + List.length constructor_type_hyps + List.length c_scrutinee_ctx),
+                                        [|EConstr.mkRel (1 + List.length constructor_type_hyps + 6)|]
+                                      ))
+                                      (EConstr.mkApp (
+                                        c_scrutinee_encoder.encoder_encode |> EConstr.Vars.lift (1 + List.length constructor_type_hyps + List.length c_scrutinee_ctx),
+                                        [|constructor_app |> EConstr.Vars.lift 1|]
+                                      ))
+                                      (EConstr.mkRel (1 + List.length constructor_type_hyps + 3))
+                                      (EConstr.mkRel 1);
+                                    EConstr.mkRel (1 + List.length constructor_type_hyps + 4);
+                                    EConstr.mkRel (1 + List.length constructor_type_hyps + 5);
+                                    constructor_app |> EConstr.Vars.lift 1;
+                                  ]
+                                )
+                            )
+                          )
+                        ) constructor_types_hyps_concl c_brs c_brs_t_compilation
+                      ),
+                      [|mk_eq_refl env
+                        (mk_vector_type env
+                          (mk_bool_type env)
+                          (c_scrutinee_encoder.encoder_len |> EConstr.Vars.lift (List.length c_scrutinee_ctx)))
+                        (EConstr.mkApp (
+                          c_scrutinee_encoder.encoder_encode |> EConstr.Vars.lift (List.length c_scrutinee_ctx),
+                          [|EConstr.mkRel 6|]
+                        ))|]
+                    ) in
+                  Feedback.msg_info Pp.(str "AAA" ++ spc () ++ Printer.pr_econstr_env env sigma c_brs_t_compilation.(0).compilation_eval_circuit);
+                  Feedback.msg_info Pp.(str "HEY_4" ++ spc () ++ Printer.pr_econstr_env env sigma c_compilation_gen_eval_circuit);
+                  let c_compilation_gen_circuit_erased_all =
+                    Array.map2 (fun (constructor_type_hyps, _) br_t_compilation ->
+                      br_t_compilation.compilation_circuit_erased
+                        |> econstr_substl_opt sigma (constructor_type_hyps |> List.map (fun _ -> None))
+                    ) constructor_types_hyps_concl c_brs_t_compilation in
+                  let c_compilation_gen_circuit_erased = c_compilation_gen_circuit_erased_all.(0) in
+                  (* assert (c_compilation_gen_circuit_erased_all |> Array.for_all (EConstr.eq_constr sigma c_compilation_gen_circuit_erased)); *)
+                  Feedback.msg_info Pp.(str "HEY_5" ++ spc () ++ Printer.pr_econstr_env env sigma c_compilation_gen_circuit_erased);
+                  let c_compilation_gen_eq_circuit_erased_all =
+                    Array.map2 (fun (constructor_type_hyps, _) br_t_compilation ->
+                      br_t_compilation.compilation_eq_circuit_erased
+                        |> econstr_substl_opt sigma (constructor_type_hyps |> List.map (fun _ -> None))
+                    ) constructor_types_hyps_concl c_brs_t_compilation in
+                  let c_compilation_gen_eq_circuit_erased = c_compilation_gen_eq_circuit_erased_all.(0) in
+                  (* assert (c_compilation_gen_eq_circuit_erased_all |> Array.for_all (EConstr.eq_constr sigma c_compilation_gen_eq_circuit_erased)); *)
+                  Feedback.msg_info Pp.(str "HEY_6" ++ spc () ++ Printer.pr_econstr_env env sigma c_compilation_gen_eq_circuit_erased);
+                  let c_scrutinee_compilation_subst =
+                    [
+                      c_scrutinee_compilation.compilation_eq_circuit_erased;
+                      c_scrutinee_compilation.compilation_circuit_erased;
+                      c_scrutinee_compilation.compilation_eval_circuit;
+                      c_scrutinee_compilation.compilation_wf_circuit;
+                      c_scrutinee_compilation.compilation_circuit;
+                      c_scrutinee_compilation.compilation_orig;
+                    ] in
+                  Seq.return (
+                    ReprTransformed,
+                    {
+                      compilation_orig =
+                        c_compilation_gen_orig
+                          |> EConstr.Vars.substl c_scrutinee_compilation_subst;
+                      compilation_circuit =
+                        c_compilation_gen_circuit
+                          |> EConstr.Vars.substl c_scrutinee_compilation_subst;
+                      compilation_wf_circuit =
+                        c_compilation_gen_wf_circuit
+                          |> EConstr.Vars.substl c_scrutinee_compilation_subst;
+                      compilation_eval_circuit =
+                        c_compilation_gen_eval_circuit
+                          |> EConstr.Vars.substl c_scrutinee_compilation_subst;
+                      compilation_circuit_erased =
+                        c_compilation_gen_circuit_erased
+                          |> EConstr.Vars.substl c_scrutinee_compilation_subst;
+                      compilation_eq_circuit_erased =
+                        c_compilation_gen_eq_circuit_erased
+                          |> EConstr.Vars.substl c_scrutinee_compilation_subst;
+                    }
                   )
-              )
+                )
+              | None -> Seq.empty
+            else if c_scrutinee_repr = ReprRaw then
+              enumerate_reprs
+                (env |> EConstr.push_rel_context (Context.Rel.Declaration.LocalAssum (EConstr.anonR, scrutinee_type_arity_ctx) :: arity_ctx))
+                sigma
+                (None :: (arity_ctx |> List.map (fun _ -> None)) @ (context_encoders |> List.map (Option.map (encoder_lift (1 + List.length arity_ctx)))))
+                c_return_t
+                |> List.to_seq
+                |> Seq.flat_map (fun c_return_t_repr ->
+                  let c_return_t_compilation_type =
+                    get_compilation_type
+                      (env |> EConstr.push_rel_context (Context.Rel.Declaration.LocalAssum (EConstr.anonR, scrutinee_type_arity_ctx) :: arity_ctx))
+                      sigma
+                      (None :: (arity_ctx |> List.map (fun _ -> None)) @ (context_encoders |> List.map (Option.map (encoder_lift (1 + List.length arity_ctx)))))
+                      (input_encoder |> encoder_lift (1 + List.length arity_ctx))
+                      c_return_t
+                      c_return_t_repr in
+                  Array.map2 (fun (c_br_annots, c_br_t) (constructor_type_ctx, _) ->
+                    create_compilations
+                      (env |> EConstr.push_rel_context constructor_type_ctx)
+                      sigma
+                      ((constructor_type_ctx |> List.map (fun _ -> None)) @ (context_encoders |> List.map (Option.map (encoder_lift (List.length constructor_type_ctx)))))
+                      ((constructor_type_ctx |> List.map (fun _ -> ReprRaw)) @ context_reprs)
+                      ((constructor_type_ctx |> List.map (fun _ -> None)) @ (context_compilations |> List.map (Option.map (compilation_lift (List.length constructor_type_ctx)))))
+                      (input_encoder |> encoder_lift (List.length constructor_type_ctx))
+                      c_br_t
+                    |> Seq.filter_map (fun (c_br_t_repr, c_br_t_compilation) ->
+                      if c_br_t_repr = c_return_t_repr then Some (c_br_annots, c_br_t_compilation) else None
+                    )
+                  ) c_brs constructor_types_ctx_concl
+                    |> seq_product_array
+                    |> Seq.flat_map (fun c_brs_annots_t_compilation ->
+                      let c_compilation_gen_orig =
+                        EConstr.mkCase (
+                          ci,
+                          u,
+                          c_params |> Array.map (EConstr.Vars.lift (1 + List.length arity_ctx)),
+                          (
+                            (
+                              c_return_annots,
+                              c_return_t_compilation_type.compilation_orig
+                                |> EConstr.Vars.liftn (1 + List.length arity_ctx) (0 + 1 + List.length arity_ctx + 1)
+                                |> EConstr.Vars.substl []
+                            ),
+                            EConstr.ERelevance.relevant
+                          ),
+                          Constr.NoInvert,
+                          EConstr.mkRel 1,
+                          c_brs_annots_t_compilation |> Array.map (fun (c_br_annots, c_br_t_compilation) ->
+                            (
+                              c_br_annots,
+                              c_br_t_compilation.compilation_orig
+                                |> EConstr.Vars.liftn (1 + List.length arity_ctx) (Array.length c_br_annots + 1)
+                            )
+                          )
+                        ) in
+                      let c_compilation_gen_circuit =
+                        EConstr.mkCase (
+                          ci,
+                          u,
+                          c_params |> Array.map (EConstr.Vars.lift (1 + List.length arity_ctx)),
+                          (
+                            (
+                              c_return_annots,
+                              c_return_t_compilation_type.compilation_circuit
+                                |> EConstr.Vars.liftn (1 + List.length arity_ctx) (1 + 1 + List.length arity_ctx + 1)
+                                |> EConstr.Vars.substl [
+                                  c_compilation_gen_orig
+                                    |> EConstr.Vars.liftn (1 + List.length arity_ctx) (1 + List.length arity_ctx + 1);
+                                ]
+                            ),
+                            EConstr.ERelevance.relevant
+                          ),
+                          Constr.NoInvert,
+                          EConstr.mkRel 1,
+                          c_brs_annots_t_compilation |> Array.map (fun (c_br_annots, c_br_t_compilation) ->
+                            (
+                              c_br_annots,
+                              c_br_t_compilation.compilation_circuit
+                                |> EConstr.Vars.liftn (1 + List.length arity_ctx) (Array.length c_br_annots + 1)
+                            )
+                          )
+                        ) in
+                      let c_compilation_gen_wf_circuit =
+                        EConstr.mkCase (
+                          ci,
+                          u,
+                          c_params |> Array.map (EConstr.Vars.lift (1 + List.length arity_ctx)),
+                          (
+                            (
+                              c_return_annots,
+                              c_return_t_compilation_type.compilation_wf_circuit
+                                |> EConstr.Vars.liftn (1 + List.length arity_ctx) (2 + 1 + List.length arity_ctx + 1)
+                                |> EConstr.Vars.substl [
+                                  c_compilation_gen_circuit
+                                    |> EConstr.Vars.liftn (1 + List.length arity_ctx) (1 + List.length arity_ctx + 1);
+                                  c_compilation_gen_orig
+                                    |> EConstr.Vars.liftn (1 + List.length arity_ctx) (1 + List.length arity_ctx + 1);
+                                ]
+                            ),
+                            EConstr.ERelevance.relevant
+                          ),
+                          Constr.NoInvert,
+                          EConstr.mkRel 1,
+                          c_brs_annots_t_compilation |> Array.map (fun (c_br_annots, c_br_t_compilation) ->
+                            (
+                              c_br_annots,
+                              c_br_t_compilation.compilation_wf_circuit
+                                |> EConstr.Vars.liftn (1 + List.length arity_ctx) (Array.length c_br_annots + 1)
+                            )
+                          )
+                        ) in
+                      let c_compilation_gen_eval_circuit =
+                        EConstr.mkCase (
+                          ci,
+                          u,
+                          c_params |> Array.map (EConstr.Vars.lift (1 + List.length arity_ctx)),
+                          (
+                            (
+                              c_return_annots,
+                              c_return_t_compilation_type.compilation_eval_circuit
+                                |> EConstr.Vars.liftn (1 + List.length arity_ctx) (3 + 1 + List.length arity_ctx + 1)
+                                |> EConstr.Vars.substl [
+                                  c_compilation_gen_wf_circuit
+                                    |> EConstr.Vars.liftn (1 + List.length arity_ctx) (1 + List.length arity_ctx + 1);
+                                  c_compilation_gen_circuit
+                                    |> EConstr.Vars.liftn (1 + List.length arity_ctx) (1 + List.length arity_ctx + 1);
+                                  c_compilation_gen_orig
+                                    |> EConstr.Vars.liftn (1 + List.length arity_ctx) (1 + List.length arity_ctx + 1);
+                                ]
+                            ),
+                            EConstr.ERelevance.relevant
+                          ),
+                          Constr.NoInvert,
+                          EConstr.mkRel 1,
+                          c_brs_annots_t_compilation |> Array.map (fun (c_br_annots, c_br_t_compilation) ->
+                            (
+                              c_br_annots,
+                              c_br_t_compilation.compilation_eval_circuit
+                                |> EConstr.Vars.liftn (1 + List.length arity_ctx) (Array.length c_br_annots + 1)
+                            )
+                          )
+                        ) in
+                      let c_compilation_gen_circuit_erased =
+                        EConstr.mkCase (
+                          ci,
+                          u,
+                          c_params |> Array.map (EConstr.Vars.lift (1 + List.length arity_ctx)),
+                          (
+                            (
+                              c_return_annots,
+                              c_return_t_compilation_type.compilation_circuit_erased
+                                |> EConstr.Vars.liftn (1 + List.length arity_ctx) (4 + 1 + List.length arity_ctx + 1)
+                                |> EConstr.Vars.substl [
+                                  c_compilation_gen_eval_circuit
+                                    |> EConstr.Vars.liftn (1 + List.length arity_ctx) (1 + List.length arity_ctx + 1);
+                                  c_compilation_gen_wf_circuit
+                                    |> EConstr.Vars.liftn (1 + List.length arity_ctx) (1 + List.length arity_ctx + 1);
+                                  c_compilation_gen_circuit
+                                    |> EConstr.Vars.liftn (1 + List.length arity_ctx) (1 + List.length arity_ctx + 1);
+                                  c_compilation_gen_orig
+                                    |> EConstr.Vars.liftn (1 + List.length arity_ctx) (1 + List.length arity_ctx + 1);
+                                ]
+                            ),
+                            EConstr.ERelevance.relevant
+                          ),
+                          Constr.NoInvert,
+                          EConstr.mkRel 1,
+                          c_brs_annots_t_compilation |> Array.map (fun (c_br_annots, c_br_t_compilation) ->
+                            (
+                              c_br_annots,
+                              c_br_t_compilation.compilation_circuit_erased
+                                |> EConstr.Vars.liftn (1 + List.length arity_ctx) (Array.length c_br_annots + 1)
+                            )
+                          )
+                        ) in
+                      let c_compilation_gen_eq_circuit_erased =
+                        EConstr.mkCase (
+                          ci,
+                          u,
+                          c_params |> Array.map (EConstr.Vars.lift (1 + List.length arity_ctx)),
+                          (
+                            (
+                              c_return_annots,
+                              c_return_t_compilation_type.compilation_eq_circuit_erased
+                                |> EConstr.Vars.liftn (1 + List.length arity_ctx) (5 + 1 + List.length arity_ctx + 1)
+                                |> EConstr.Vars.substl [
+                                  c_compilation_gen_circuit_erased
+                                    |> EConstr.Vars.liftn (1 + List.length arity_ctx) (1 + List.length arity_ctx + 1);
+                                  c_compilation_gen_eval_circuit
+                                    |> EConstr.Vars.liftn (1 + List.length arity_ctx) (1 + List.length arity_ctx + 1);
+                                  c_compilation_gen_wf_circuit
+                                    |> EConstr.Vars.liftn (1 + List.length arity_ctx) (1 + List.length arity_ctx + 1);
+                                  c_compilation_gen_circuit
+                                    |> EConstr.Vars.liftn (1 + List.length arity_ctx) (1 + List.length arity_ctx + 1);
+                                  c_compilation_gen_orig
+                                    |> EConstr.Vars.liftn (1 + List.length arity_ctx) (1 + List.length arity_ctx + 1);
+                                ]
+                            ),
+                            EConstr.ERelevance.relevant
+                          ),
+                          Constr.NoInvert,
+                          EConstr.mkRel 1,
+                          c_brs_annots_t_compilation |> Array.map (fun (c_br_annots, c_br_t_compilation) ->
+                            (
+                              c_br_annots,
+                              c_br_t_compilation.compilation_eq_circuit_erased
+                                |> EConstr.Vars.liftn (1 + List.length arity_ctx) (Array.length c_br_annots + 1)
+                            )
+                          )
+                        ) in
+                      Seq.return (
+                        c_return_t_repr,
+                        {
+                          compilation_orig =
+                            c_compilation_gen_orig
+                              |> econstr_substl_opt sigma (Some c_scrutinee_compilation.compilation_orig :: (arity_ctx |> List.map (fun _ -> None)));
+                          compilation_circuit =
+                            c_compilation_gen_circuit
+                              |> econstr_substl_opt sigma (Some c_scrutinee_compilation.compilation_orig :: (arity_ctx |> List.map (fun _ -> None)));
+                          compilation_wf_circuit =
+                            c_compilation_gen_wf_circuit
+                              |> econstr_substl_opt sigma (Some c_scrutinee_compilation.compilation_orig :: (arity_ctx |> List.map (fun _ -> None)));
+                          compilation_eval_circuit =
+                            c_compilation_gen_eval_circuit
+                              |> econstr_substl_opt sigma (Some c_scrutinee_compilation.compilation_orig :: (arity_ctx |> List.map (fun _ -> None)));
+                          compilation_circuit_erased =
+                            c_compilation_gen_circuit_erased
+                              |> econstr_substl_opt sigma (Some c_scrutinee_compilation.compilation_orig :: (arity_ctx |> List.map (fun _ -> None)));
+                          compilation_eq_circuit_erased =
+                            c_compilation_gen_eq_circuit_erased
+                              |> econstr_substl_opt sigma (Some c_scrutinee_compilation.compilation_orig :: (arity_ctx |> List.map (fun _ -> None)));
+                        }
+                      )
+                    )
+                )
+              else
+                Seq.empty
           )
       else
         Seq.empty)
